QCP/SeparationLogic/SeparationLogic/ArrayLib.v
@@ -7,10 +7,10 @@ Require Import Coq.Classes.RelationClasses.
 Require Import Coq.Classes.Morphisms.
 Require Import Coq.micromega.Psatz.
 Require Import Coq.Sorting.Permutation.
-From AUXLib Require Import int_auto Axioms Feq Idents List_lemma VMap.
+From AUXLib Require Import int_auto Axioms Feq Idents List_lemma VMap ListLib.
 From compcert.lib Require Import Integers.
 Require Import SetsClass.SetsClass. Import SetsNotation.
-From SimpleC.SL Require Import Mem CommonAssertion ListLib StoreAux.
+From SimpleC.SL Require Import Mem CommonAssertion StoreAux.
 Require Import Logic.LogicGenerator.demo932.Interface.
 Local Open Scope Z_scope.
 Local Open Scope sets.
@@ -524,6 +524,268 @@ Lemma store_int_array_divide_rec:
 Proof.
   intros; unfold store_int_array, store_array. 
   eapply store_array_rec_divide with (storeA := store_int); eauto.
+Qed.
+
+Definition store_uint_array_rec (x: addr) (lo hi: Z) (l: list Z): Assertion :=
+  store_array_rec (fun x lo a => (x + lo * sizeof(UINT)) # UInt |-> a) x lo hi l.
+  
+Definition store_undef_uint_array_rec (x: addr) (lo hi: Z): Assertion :=
+  store_undef_array_rec (fun x lo => (x + lo * sizeof(UINT)) # UInt |->_ ) x lo hi (Z.to_nat (hi - lo)).
+
+Lemma store_uint_array_rec_length: forall x lo hi l,
+  store_uint_array_rec x lo hi l |-- [| Z.of_nat (length l) = hi - lo |].
+Proof.
+  intros.
+  unfold store_uint_array_rec.
+  sep_apply (store_array_rec_length (fun x lo a => (x + lo * sizeof(UINT)) # UInt |-> a)). entailer!.
+Qed.
+
+Lemma store_uint_array_rec_Zlength: forall x lo hi l,
+  store_uint_array_rec x lo hi l |-- [| Zlength l = hi - lo |].
+Proof.
+  intros.
+  sep_apply store_uint_array_rec_length.
+  rewrite Zlength_correct.
+  entailer!.
+Qed.
+
+
+Definition store_uint_array_missing_i_rec (x: addr) (i lo hi: Z) (l: list Z): Assertion := 
+  store_array_missing_i_rec (fun x lo a => (x + lo * sizeof(UINT)) # UInt |-> a) x i lo hi l.
+
+Definition store_undef_uint_array_missing_i_re (x: addr) (i lo hi: Z) : Assertion :=
+  store_undef_array_missing_i_rec (fun x lo => (x + lo * sizeof(UINT)) # UInt |->_ ) x i lo hi (Z.to_nat (hi - lo)).
+
+Definition store_uint_array (x: addr) (n: Z) (l: list Z): Assertion :=
+  store_array (fun x lo a => (x + lo * sizeof(UINT)) # UInt |-> a) x n l.
+
+Definition store_undef_uint_array (x: addr) (n: Z): Assertion :=
+  store_undef_array (fun x lo => (x + lo * sizeof(UINT)) # UInt |->_ ) x n.
+
+Lemma store_uint_array_length: forall x n l,
+  store_uint_array x n l |-- [| Z.of_nat (length l) = n |].
+Proof.
+  intros.
+  unfold store_uint_array.
+  sep_apply store_uint_array_rec_length.
+  entailer!. 
+Qed.
+
+Lemma store_uint_array_Zlength: forall x n l,
+  store_uint_array x n l |-- [| Zlength l = n |].
+Proof.
+  intros.
+  unfold store_uint_array.
+  apply store_array_Zlength.
+Qed.
+
+Lemma store_uint_array_range : forall x n l,
+  store_uint_array x n l |-- [| forall a, In a l -> NULL <= a <= Int.max_unsigned |].
+Proof.
+  intros.
+  unfold store_uint_array.
+  unfold store_array.
+  remember 0 as lo. 
+  rename n into hi.
+  clear Heqlo. revert lo hi. unfold NULL. 
+  induction l ; intros. 
+  - entailer!.
+  - simpl. prop_apply IHl.
+    prop_apply store_uint_range.
+    entailer!.
+    intros. destruct H1 ; auto.
+    subst. auto. 
+Qed.
+
+Lemma store_uint_array_rec_split: forall x lo n m l,
+  lo <= n < m ->
+  store_uint_array_rec x lo m l |-- store_uint (x + n * sizeof(UINT)) (Znth (n -lo) l 0) ** store_uint_array_missing_i_rec x n lo m l.
+Proof.
+  intros.
+  unfold store_uint_array_rec, store_uint_array_missing_i_rec.
+  sep_apply (store_array_rec_split (fun x lo a => (x + lo * sizeof(UINT)) # UInt |-> a)). entailer!.
+  lia.
+Qed.
+
+Lemma store_uint_array_rec_merge: forall x lo n m a l,
+  lo <= n < m ->
+  store_uint (x + n * sizeof(UINT)) a ** store_uint_array_missing_i_rec x n lo m l |-- store_uint_array_rec x lo m (replace_Znth (n -lo) a l).
+Proof.
+  intros.
+  unfold store_uint_array_rec, store_uint_array_missing_i_rec.
+  sep_apply (store_array_rec_merge (fun x lo a => (x + lo * sizeof(UINT)) # UInt |-> a)). entailer!.
+  lia.
+Qed.
+
+Lemma store_uint_array_rec_divide:
+  forall x lo n l m,
+    lo <= m <= n -> Zlength l = n -lo ->
+    store_uint_array_rec x lo n l --||-- 
+    store_uint_array_rec x lo m (sublist 0 (m - lo) l) ** store_uint_array_rec x m n (sublist (m -lo) (n -lo) l).
+Proof.
+  intros; unfold store_uint_array_rec. 
+  eapply store_array_rec_divide_aux with (storeA := store_uint); eauto.
+Qed.
+
+Lemma store_uint_array_rec_divide_rev:
+  forall x lo n l1 l2 m,
+    lo <= m <= n -> 
+    store_uint_array_rec x lo m l1 ** store_uint_array_rec x m n l2 |-- 
+    store_uint_array_rec x lo n (l1 ++ l2).
+Proof.
+  intros.
+  prop_apply (store_uint_array_rec_Zlength x lo).
+  prop_apply (store_uint_array_rec_Zlength x m).
+  Intros.
+  rewrite (store_uint_array_rec_divide x lo n (l1 ++ l2) m);[ | lia | ].
+  rewrite <- H0.
+  rewrite sublist_app_exact1 by lia.
+  rewrite sublist_split_app_r with (len := Zlength l1) by lia.
+  replace (Zlength l1 - Zlength l1) with 0 by lia.
+  rewrite sublist_self by lia.
+  entailer!.
+  rewrite Zlength_app. lia.
+Qed.
+
+Lemma store_uint_array_rec_head:
+  forall x lo hi l,
+    lo < hi -> 
+    store_uint_array_rec x lo hi l  |-- 
+    (x + lo * sizeof ( UINT )) # UInt |-> (Znth 0 l 0) ** 
+    store_uint_array_rec x (lo + 1) hi (sublist 1 (hi - lo) l).
+Proof.
+  intros.
+  destruct l.
+  - unfold store_uint_array_rec. simpl.
+    entailer!.
+  - prop_apply (store_uint_array_rec_Zlength x lo hi).
+  Intros.
+  rewrite (store_uint_array_rec_divide x lo hi ((z :: nil) ++ l) (lo + 1));[ | lia | easy ].
+  replace (lo + 1 - lo) with 1 by lia.
+  assert (Zlength (z::nil) = 1). { rewrite Zlength_cons, Zlength_nil. lia. }
+  rewrite <- H1 at 2.
+  rewrite sublist_app_exact1.
+  replace (z::l) with (app (z :: nil) l)  by easy.
+  rewrite sublist_split_app_r with (len := 1) by lia.
+  replace (1 - 1) with 0 by lia.
+  rewrite sublist_self.
+  entailer!.
+  unfold store_uint_array_rec. simpl.
+  Intros.
+  rewrite Znth0_cons.
+  entailer!.
+  rewrite Zlength_cons in H0. lia. 
+Qed.
+
+
+Lemma store_uint_array_rec_head_merge:
+  forall x lo hi z l,
+    lo < hi -> 
+    (x + lo * sizeof ( UINT )) # UInt |-> z ** 
+    store_uint_array_rec x (lo + 1) hi l |-- 
+    store_uint_array_rec x lo hi (z :: l).
+Proof.
+  intros.
+  prop_apply (store_uint_array_rec_Zlength x (lo + 1) hi).
+  Intros.
+  rewrite (store_uint_array_rec_divide x lo hi ((z :: nil) ++ l) (lo + 1));[ | lia |  ].
+  replace (lo + 1 - lo) with 1 by lia.
+  assert (Zlength (z::nil) = 1). { rewrite Zlength_cons, Zlength_nil. lia. }
+  rewrite <- H1 at 3.
+  rewrite sublist_app_exact1.
+  rewrite sublist_split_app_r with (len := 1) by lia.
+  replace (1 - 1) with 0 by lia.
+  rewrite sublist_self by lia.
+  entailer!.
+  unfold store_uint_array_rec. simpl.
+  entailer!.
+  rewrite Zlength_app, Zlength_cons, Zlength_nil.  lia. 
+Qed.
+
+Lemma store_uint_array_rec_tail_merge:
+  forall x lo hi z l,
+    lo <= hi -> 
+    (x + hi * sizeof ( UINT )) # UInt |-> z ** 
+    store_uint_array_rec x lo hi l |-- 
+    store_uint_array_rec x lo (hi + 1) (l ++ [z]).
+Proof.
+  intros.
+  prop_apply (store_uint_array_rec_Zlength x lo hi).
+  Intros.
+  rewrite (store_uint_array_rec_divide x lo (hi + 1) (l ++ [z]) hi);[ | lia |  ].
+  rewrite <- H0 at 1.
+  rewrite sublist_app_exact1.
+  rewrite sublist_split_app_r with (len := hi - lo) by lia.
+  replace (hi - lo - (hi - lo)) with 0 by lia.
+  rewrite sublist_self.
+  entailer!.
+  unfold store_uint_array_rec. simpl.
+  entailer!.
+  rewrite Zlength_cons, Zlength_nil. lia.
+  rewrite Zlength_app, Zlength_cons, Zlength_nil.  lia. 
+Qed.
+
+Lemma store_uint_array_rec_cons:
+  forall x lo hi z l,
+    lo < hi -> 
+    store_uint_array_rec x lo hi (z::l)  |-- 
+    (x + lo * sizeof ( UINT )) # UInt |-> z ** 
+    store_uint_array_rec x (lo + 1) hi l.
+Proof.
+  intros.
+  prop_apply store_uint_array_rec_Zlength.
+  Intros.
+  rewrite Zlength_cons in H0.
+  sep_apply store_uint_array_rec_head;[ | lia].
+  rewrite Znth0_cons.
+  replace (z :: l) with ([z] ++ l) by easy.
+  rewrite sublist_split_app_r with (len := 1).
+  replace (1-1) with 0 by lia.
+  rewrite sublist_self by lia.
+  entailer!.
+  rewrite Zlength_cons,Zlength_nil. lia.
+  lia.
+Qed.
+
+Lemma store_uint_array_split: forall x n m l,
+  0 <= n < m ->
+  store_uint_array x m l |-- store_uint (x + n * sizeof(UINT)) (Znth n l 0) ** store_uint_array_missing_i_rec x n 0 m l.
+Proof.
+  intros.
+  unfold store_uint_array, store_uint_array_missing_i_rec.
+  sep_apply (store_array_split (fun x lo a => (x + lo * sizeof(UINT)) # UInt |-> a)). entailer!.
+  lia.
+Qed.
+
+Lemma store_uint_array_merge: forall x n m a l,
+  0 <= n < m ->
+  store_uint (x + n * sizeof(UINT)) a ** store_uint_array_missing_i_rec x n 0 m l |-- store_uint_array x m (replace_Znth n a l).
+Proof.
+  intros.
+  unfold store_uint_array, store_uint_array_missing_i_rec.
+  sep_apply (store_array_merge (fun x lo a => (x + lo * sizeof(UINT)) # UInt |-> a)). entailer!.
+  lia.
+Qed.
+
+Lemma store_uint_array_divide:
+  forall x n l m,
+    0 <= m <= n -> Zlength l = n ->
+    store_uint_array x n l --||-- 
+    store_uint_array x m (sublist 0 m l) ** store_uint_array (x + m*sizeof(UINT)) (n-m) (sublist m n l).
+Proof.
+  intros; unfold store_uint_array. 
+  eapply store_array_divide with (storeA := store_uint); eauto.
+  auto.
+Qed.
+
+Lemma store_uint_array_divide_rec:
+  forall x n l m,
+    0 <= m <= n -> Zlength l = n ->
+    store_uint_array x n l --||-- 
+    store_uint_array_rec x 0 m (sublist 0 m l) ** store_uint_array_rec x m n (sublist m n l).
+Proof.
+  intros; unfold store_uint_array, store_array. 
+  eapply store_array_rec_divide with (storeA := store_uint); eauto.
 Qed.
 
 End IntArrayLib.
