QCP/SeparationLogic/examples/fme/fme_goal.v
@@ -18,8 +18,8 @@ Import naive_C_Rules.
 Require Import fme_lib.
 Import naive_C_Rules.
 Local Open Scope sac.
-From SimpleC.EE Require Import common_strategy_goal.
-From SimpleC.EE Require Import common_strategy_proof.
+Require Import common_strategy_goal.
+Require Import common_strategy_proof.
 Require Import fme_strategy_goal.
 Require Import fme_strategy_proof.
 
@@ -298,7 +298,8 @@ Definition NilInequList_return_wit_1 :=
 
 Definition ConsInequList_return_wit_1 := 
 forall (l_pre: Z) (c_pre: Z) (l0: (@list Constraint)) (c0: Constraint) (n: Z) (retval: Z) ,
-  [| (retval <> 0) |]
+  [| (retval <> 0) |] 
+  &&  [| (c_pre <> 0) |]
   &&  ((&((retval)  # "InequList" ->ₛ "coef")) # Ptr  |-> c_pre)
   **  ((&((retval)  # "InequList" ->ₛ "next")) # Ptr  |-> l_pre)
   **  (coef_array c_pre n c0 )
@@ -309,10 +310,12 @@ forall (l_pre: Z) (c_pre: Z) (l0: (@list Constraint)) (c0: Constraint) (n: Z) (r
 
 Definition ConsInequList_partial_solve_wit_1 := 
 forall (l_pre: Z) (c_pre: Z) (l0: (@list Constraint)) (c0: Constraint) (n: Z) ,
-  (coef_array c_pre n c0 )
+  [| (c_pre <> 0) |]
+  &&  (coef_array c_pre n c0 )
   **  (InequList l_pre n l0 )
 |--
-  (coef_array c_pre n c0 )
+  [| (c_pre <> 0) |]
+  &&  (coef_array c_pre n c0 )
   **  (InequList l_pre n l0 )
 .
 
@@ -329,7 +332,8 @@ forall (p_pre: Z) (l: (@list Constraint)) (n: Z) ,
 
 Definition free_InequList_safety_wit_2 := 
 forall (p_pre: Z) (l: (@list Constraint)) (n: Z) (x: Constraint) (l0: (@list Constraint)) (y: Z) (h: Z) ,
-  [| (l = (cons (x) (l0))) |] 
+  [| (h <> 0) |] 
+  &&  [| (l = (cons (x) (l0))) |] 
   &&  [| (p_pre <> 0) |]
   &&  ((&((p_pre)  # "InequList" ->ₛ "coef")) # Ptr  |-> h)
   **  (InequList y n l0 )
@@ -343,27 +347,28 @@ forall (p_pre: Z) (l: (@list Constraint)) (n: Z) (x: Constraint) (l0: (@list Con
 
 Definition free_InequList_safety_wit_3 := 
 forall (p_pre: Z) (l: (@list Constraint)) (n: Z) (x: Constraint) (l0: (@list Constraint)) (y: Z) (h: Z) ,
-  [| (h <> 0) |] 
-  &&  [| (l = (cons (x) (l0))) |] 
-  &&  [| (p_pre <> 0) |]
-  &&  ((&((p_pre)  # "InequList" ->ₛ "coef")) # Ptr  |-> h)
-  **  (InequList y n l0 )
-  **  ((&((p_pre)  # "InequList" ->ₛ "next")) # Ptr  |-> y)
-  **  ((( &( "p" ) )) # Ptr  |-> p_pre)
-|--
-  [| (0 <= INT_MAX) |] 
-  &&  [| ((INT_MIN) <= 0) |]
-.
-
-Definition free_InequList_safety_wit_4 := 
-forall (p_pre: Z) (l: (@list Constraint)) (n: Z) (x: Constraint) (l0: (@list Constraint)) (y: Z) (h: Z) ,
   [| (h = 0) |] 
+  &&  [| (h <> 0) |] 
   &&  [| (l = (cons (x) (l0))) |] 
   &&  [| (p_pre <> 0) |]
   &&  ((&((p_pre)  # "InequList" ->ₛ "coef")) # Ptr  |-> h)
   **  (InequList y n l0 )
   **  ((&((p_pre)  # "InequList" ->ₛ "next")) # Ptr  |-> y)
   **  (coef_array h n x )
+  **  ((( &( "p" ) )) # Ptr  |-> p_pre)
+|--
+  [| False |]
+.
+
+Definition free_InequList_safety_wit_4 := 
+forall (p_pre: Z) (l: (@list Constraint)) (n: Z) (x: Constraint) (l0: (@list Constraint)) (y: Z) (h: Z) ,
+  [| (h <> 0) |] 
+  &&  [| (h <> 0) |] 
+  &&  [| (l = (cons (x) (l0))) |] 
+  &&  [| (p_pre <> 0) |]
+  &&  ((&((p_pre)  # "InequList" ->ₛ "coef")) # Ptr  |-> h)
+  **  (InequList y n l0 )
+  **  ((&((p_pre)  # "InequList" ->ₛ "next")) # Ptr  |-> y)
   **  ((( &( "p" ) )) # Ptr  |-> p_pre)
 |--
   [| (0 <= INT_MAX) |] 
@@ -379,19 +384,9 @@ forall (p_pre: Z) (l: (@list Constraint)) (n: Z) ,
 .
 
 Definition free_InequList_return_wit_2_1 := 
-forall (p_pre: Z) (l: (@list Constraint)) (n: Z) (x: Constraint) (l0: (@list Constraint)) (y: Z) (h: Z) ,
-  [| (y <> 0) |] 
-  &&  [| (h = 0) |] 
-  &&  [| (l = (cons (x) (l0))) |] 
-  &&  [| (p_pre <> 0) |]
-  &&  (coef_array h n x )
-|--
-  TT && emp 
-.
-
-Definition free_InequList_return_wit_2_2 := 
 forall (p_pre: Z) (l: (@list Constraint)) (x: Constraint) (l0: (@list Constraint)) (y: Z) (h: Z) ,
   [| (y <> 0) |] 
+  &&  [| (h <> 0) |] 
   &&  [| (h <> 0) |] 
   &&  [| (l = (cons (x) (l0))) |] 
   &&  [| (p_pre <> 0) |]
@@ -400,25 +395,14 @@ forall (p_pre: Z) (l: (@list Constraint)) (x: Constraint) (l0: (@list Constraint
   TT && emp 
 .
 
-Definition free_InequList_return_wit_2_3 := 
+Definition free_InequList_return_wit_2_2 := 
 forall (p_pre: Z) (l: (@list Constraint)) (n: Z) (x: Constraint) (l0: (@list Constraint)) (y: Z) (h: Z) ,
   [| (y = 0) |] 
+  &&  [| (h <> 0) |] 
   &&  [| (h <> 0) |] 
   &&  [| (l = (cons (x) (l0))) |] 
   &&  [| (p_pre <> 0) |]
   &&  (InequList y n l0 )
-|--
-  TT && emp 
-.
-
-Definition free_InequList_return_wit_2_4 := 
-forall (p_pre: Z) (l: (@list Constraint)) (n: Z) (x: Constraint) (l0: (@list Constraint)) (y: Z) (h: Z) ,
-  [| (y = 0) |] 
-  &&  [| (h = 0) |] 
-  &&  [| (l = (cons (x) (l0))) |] 
-  &&  [| (p_pre <> 0) |]
-  &&  (InequList y n l0 )
-  **  (coef_array h n x )
 |--
   TT && emp 
 .
@@ -429,7 +413,8 @@ forall (p_pre: Z) (l: (@list Constraint)) (n: Z) ,
   &&  (InequList p_pre n l )
 |--
   EX (h: Z)  (y: Z)  (l0: (@list Constraint))  (x: Constraint) ,
-  [| (l = (cons (x) (l0))) |] 
+  [| (h <> 0) |] 
+  &&  [| (l = (cons (x) (l0))) |] 
   &&  [| (p_pre <> 0) |]
   &&  ((&((p_pre)  # "InequList" ->ₛ "coef")) # Ptr  |-> h)
   **  (InequList y n l0 )
@@ -440,6 +425,7 @@ forall (p_pre: Z) (l: (@list Constraint)) (n: Z) ,
 Definition free_InequList_partial_solve_wit_2 := 
 forall (p_pre: Z) (l: (@list Constraint)) (n: Z) (x: Constraint) (l0: (@list Constraint)) (y: Z) (h: Z) ,
   [| (h <> 0) |] 
+  &&  [| (h <> 0) |] 
   &&  [| (l = (cons (x) (l0))) |] 
   &&  [| (p_pre <> 0) |]
   &&  ((&((p_pre)  # "InequList" ->ₛ "coef")) # Ptr  |-> h)
@@ -448,6 +434,7 @@ forall (p_pre: Z) (l: (@list Constraint)) (n: Z) (x: Constraint) (l0: (@list Con
   **  (coef_array h n x )
 |--
   [| (h <> 0) |] 
+  &&  [| (h <> 0) |] 
   &&  [| (l = (cons (x) (l0))) |] 
   &&  [| (p_pre <> 0) |]
   &&  (coef_array h n x )
@@ -460,6 +447,7 @@ Definition free_InequList_partial_solve_wit_3 :=
 forall (p_pre: Z) (l: (@list Constraint)) (n: Z) (x: Constraint) (l0: (@list Constraint)) (y: Z) (h: Z) ,
   [| (y <> 0) |] 
   &&  [| (h <> 0) |] 
+  &&  [| (h <> 0) |] 
   &&  [| (l = (cons (x) (l0))) |] 
   &&  [| (p_pre <> 0) |]
   &&  ((&((p_pre)  # "InequList" ->ₛ "coef")) # Ptr  |-> h)
@@ -467,6 +455,7 @@ forall (p_pre: Z) (l: (@list Constraint)) (n: Z) (x: Constraint) (l0: (@list Con
   **  ((&((p_pre)  # "InequList" ->ₛ "next")) # Ptr  |-> y)
 |--
   [| (y <> 0) |] 
+  &&  [| (h <> 0) |] 
   &&  [| (h <> 0) |] 
   &&  [| (l = (cons (x) (l0))) |] 
   &&  [| (p_pre <> 0) |]
@@ -476,65 +465,28 @@ forall (p_pre: Z) (l: (@list Constraint)) (n: Z) (x: Constraint) (l0: (@list Con
 .
 
 Definition free_InequList_partial_solve_wit_4 := 
-forall (p_pre: Z) (l: (@list Constraint)) (n: Z) (x: Constraint) (l0: (@list Constraint)) (y: Z) (h: Z) ,
+forall (p_pre: Z) (l: (@list Constraint)) (x: Constraint) (l0: (@list Constraint)) (y: Z) (h: Z) ,
   [| (y <> 0) |] 
-  &&  [| (h = 0) |] 
+  &&  [| (h <> 0) |] 
+  &&  [| (h <> 0) |] 
   &&  [| (l = (cons (x) (l0))) |] 
   &&  [| (p_pre <> 0) |]
   &&  ((&((p_pre)  # "InequList" ->ₛ "coef")) # Ptr  |-> h)
-  **  (InequList y n l0 )
   **  ((&((p_pre)  # "InequList" ->ₛ "next")) # Ptr  |-> y)
-  **  (coef_array h n x )
 |--
   [| (y <> 0) |] 
-  &&  [| (h = 0) |] 
+  &&  [| (h <> 0) |] 
+  &&  [| (h <> 0) |] 
   &&  [| (l = (cons (x) (l0))) |] 
   &&  [| (p_pre <> 0) |]
-  &&  (InequList y n l0 )
-  **  ((&((p_pre)  # "InequList" ->ₛ "coef")) # Ptr  |-> h)
+  &&  ((&((p_pre)  # "InequList" ->ₛ "coef")) # Ptr  |-> h)
   **  ((&((p_pre)  # "InequList" ->ₛ "next")) # Ptr  |-> y)
-  **  (coef_array h n x )
 .
 
 Definition free_InequList_partial_solve_wit_5 := 
 forall (p_pre: Z) (l: (@list Constraint)) (n: Z) (x: Constraint) (l0: (@list Constraint)) (y: Z) (h: Z) ,
-  [| (y <> 0) |] 
-  &&  [| (h = 0) |] 
-  &&  [| (l = (cons (x) (l0))) |] 
-  &&  [| (p_pre <> 0) |]
-  &&  ((&((p_pre)  # "InequList" ->ₛ "coef")) # Ptr  |-> h)
-  **  ((&((p_pre)  # "InequList" ->ₛ "next")) # Ptr  |-> y)
-  **  (coef_array h n x )
-|--
-  [| (y <> 0) |] 
-  &&  [| (h = 0) |] 
-  &&  [| (l = (cons (x) (l0))) |] 
-  &&  [| (p_pre <> 0) |]
-  &&  ((&((p_pre)  # "InequList" ->ₛ "coef")) # Ptr  |-> h)
-  **  ((&((p_pre)  # "InequList" ->ₛ "next")) # Ptr  |-> y)
-  **  (coef_array h n x )
-.
-
-Definition free_InequList_partial_solve_wit_6 := 
-forall (p_pre: Z) (l: (@list Constraint)) (x: Constraint) (l0: (@list Constraint)) (y: Z) (h: Z) ,
-  [| (y <> 0) |] 
-  &&  [| (h <> 0) |] 
-  &&  [| (l = (cons (x) (l0))) |] 
-  &&  [| (p_pre <> 0) |]
-  &&  ((&((p_pre)  # "InequList" ->ₛ "coef")) # Ptr  |-> h)
-  **  ((&((p_pre)  # "InequList" ->ₛ "next")) # Ptr  |-> y)
-|--
-  [| (y <> 0) |] 
-  &&  [| (h <> 0) |] 
-  &&  [| (l = (cons (x) (l0))) |] 
-  &&  [| (p_pre <> 0) |]
-  &&  ((&((p_pre)  # "InequList" ->ₛ "coef")) # Ptr  |-> h)
-  **  ((&((p_pre)  # "InequList" ->ₛ "next")) # Ptr  |-> y)
-.
-
-Definition free_InequList_partial_solve_wit_7 := 
-forall (p_pre: Z) (l: (@list Constraint)) (n: Z) (x: Constraint) (l0: (@list Constraint)) (y: Z) (h: Z) ,
   [| (y = 0) |] 
+  &&  [| (h <> 0) |] 
   &&  [| (h <> 0) |] 
   &&  [| (l = (cons (x) (l0))) |] 
   &&  [| (p_pre <> 0) |]
@@ -544,32 +496,12 @@ forall (p_pre: Z) (l: (@list Constraint)) (n: Z) (x: Constraint) (l0: (@list Con
 |--
   [| (y = 0) |] 
   &&  [| (h <> 0) |] 
+  &&  [| (h <> 0) |] 
   &&  [| (l = (cons (x) (l0))) |] 
   &&  [| (p_pre <> 0) |]
   &&  ((&((p_pre)  # "InequList" ->ₛ "coef")) # Ptr  |-> h)
   **  ((&((p_pre)  # "InequList" ->ₛ "next")) # Ptr  |-> y)
   **  (InequList y n l0 )
-.
-
-Definition free_InequList_partial_solve_wit_8 := 
-forall (p_pre: Z) (l: (@list Constraint)) (n: Z) (x: Constraint) (l0: (@list Constraint)) (y: Z) (h: Z) ,
-  [| (y = 0) |] 
-  &&  [| (h = 0) |] 
-  &&  [| (l = (cons (x) (l0))) |] 
-  &&  [| (p_pre <> 0) |]
-  &&  ((&((p_pre)  # "InequList" ->ₛ "coef")) # Ptr  |-> h)
-  **  (InequList y n l0 )
-  **  ((&((p_pre)  # "InequList" ->ₛ "next")) # Ptr  |-> y)
-  **  (coef_array h n x )
-|--
-  [| (y = 0) |] 
-  &&  [| (h = 0) |] 
-  &&  [| (l = (cons (x) (l0))) |] 
-  &&  [| (p_pre <> 0) |]
-  &&  ((&((p_pre)  # "InequList" ->ₛ "coef")) # Ptr  |-> h)
-  **  ((&((p_pre)  # "InequList" ->ₛ "next")) # Ptr  |-> y)
-  **  (InequList y n l0 )
-  **  (coef_array h n x )
 .
 
 (*----- Function eliminate -----*)
@@ -612,6 +544,7 @@ forall (num_pre: Z) (r_pre: Z) (l: (@list Constraint)) (n: Z) (BP0: Z) (retval: 
 Definition eliminate_safety_wit_2 := 
 forall (num_pre: Z) (r_pre: Z) (l: (@list Constraint)) (n: Z) (BP0: Z) (retval: Z) (retval_2: Z) (retval_3: Z) (cur: Z) (remain: Z) (lower: Z) (upper: Z) (up: (@list Constraint)) (lo: (@list Constraint)) (re: (@list Constraint)) (bp: BP) (l1: (@list Constraint)) (l2: (@list Constraint)) (cur_next: Z) (cur_coef: Z) (x: Constraint) (l3: (@list Constraint)) ,
   [| (l2 = (cons (x) (l3))) |] 
+  &&  [| (cur_coef <> 0) |] 
   &&  [| (cur <> 0) |] 
   &&  [| (l = (app (l1) (l2))) |] 
   &&  [| (eliminate_xn (Zto_nat ((num_pre - 1 ))) l1 bp ) |] 
@@ -653,6 +586,7 @@ Definition eliminate_safety_wit_3 :=
 forall (num_pre: Z) (r_pre: Z) (l: (@list Constraint)) (n: Z) (BP0: Z) (retval: Z) (retval_2: Z) (retval_3: Z) (cur: Z) (remain: Z) (lower: Z) (upper: Z) (up: (@list Constraint)) (lo: (@list Constraint)) (re: (@list Constraint)) (bp: BP) (l1: (@list Constraint)) (l2: (@list Constraint)) (cur_next: Z) (cur_coef: Z) (x: Constraint) (l3: (@list Constraint)) ,
   [| ((coef_Znth (num_pre) (x) (0)) <> 0) |] 
   &&  [| (l2 = (cons (x) (l3))) |] 
+  &&  [| (cur_coef <> 0) |] 
   &&  [| (cur <> 0) |] 
   &&  [| (l = (app (l1) (l2))) |] 
   &&  [| (eliminate_xn (Zto_nat ((num_pre - 1 ))) l1 bp ) |] 
@@ -774,6 +708,7 @@ Definition eliminate_entail_wit_3_1 :=
 forall (num_pre: Z) (l: (@list Constraint)) (n: Z) (BP0: Z) (retval: Z) (retval_2: Z) (retval_3: Z) (cur: Z) (remain: Z) (lower: Z) (upper: Z) (up_2: (@list Constraint)) (lo_2: (@list Constraint)) (re_2: (@list Constraint)) (bp_2: BP) (l1_2: (@list Constraint)) (l2_2: (@list Constraint)) (cur_next: Z) (cur_coef: Z) (x: Constraint) (l3: (@list Constraint)) ,
   [| ((coef_Znth (num_pre) (x) (0)) = 0) |] 
   &&  [| (l2_2 = (cons (x) (l3))) |] 
+  &&  [| (cur_coef <> 0) |] 
   &&  [| (cur <> 0) |] 
   &&  [| (l = (app (l1_2) (l2_2))) |] 
   &&  [| (eliminate_xn (Zto_nat ((num_pre - 1 ))) l1_2 bp_2 ) |] 
@@ -831,6 +766,7 @@ forall (num_pre: Z) (l: (@list Constraint)) (n: Z) (BP0: Z) (retval: Z) (retval_
   [| ((coef_Znth (num_pre) (x) (0)) <= 0) |] 
   &&  [| ((coef_Znth (num_pre) (x) (0)) <> 0) |] 
   &&  [| (l2_2 = (cons (x) (l3))) |] 
+  &&  [| (cur_coef <> 0) |] 
   &&  [| (cur <> 0) |] 
   &&  [| (l = (app (l1_2) (l2_2))) |] 
   &&  [| (eliminate_xn (Zto_nat ((num_pre - 1 ))) l1_2 bp_2 ) |] 
@@ -888,6 +824,7 @@ forall (num_pre: Z) (l: (@list Constraint)) (n: Z) (BP0: Z) (retval: Z) (retval_
   [| ((coef_Znth (num_pre) (x) (0)) > 0) |] 
   &&  [| ((coef_Znth (num_pre) (x) (0)) <> 0) |] 
   &&  [| (l2_2 = (cons (x) (l3))) |] 
+  &&  [| (cur_coef <> 0) |] 
   &&  [| (cur <> 0) |] 
   &&  [| (l = (app (l1_2) (l2_2))) |] 
   &&  [| (eliminate_xn (Zto_nat ((num_pre - 1 ))) l1_2 bp_2 ) |] 
@@ -1147,6 +1084,7 @@ Definition eliminate_partial_solve_wit_4 := eliminate_partial_solve_wit_4_pure -
 Definition eliminate_partial_solve_wit_5 := 
 forall (num_pre: Z) (l: (@list Constraint)) (n: Z) (BP0: Z) (retval: Z) (retval_2: Z) (retval_3: Z) (cur: Z) (remain: Z) (lower: Z) (upper: Z) (up: (@list Constraint)) (lo: (@list Constraint)) (re: (@list Constraint)) (bp: BP) (l1: (@list Constraint)) (l2: (@list Constraint)) (cur_next: Z) (cur_coef: Z) (x: Constraint) (l3: (@list Constraint)) ,
   [| (l2 = (cons (x) (l3))) |] 
+  &&  [| (cur_coef <> 0) |] 
   &&  [| (cur <> 0) |] 
   &&  [| (l = (app (l1) (l2))) |] 
   &&  [| (eliminate_xn (Zto_nat ((num_pre - 1 ))) l1 bp ) |] 
@@ -1174,6 +1112,7 @@ forall (num_pre: Z) (l: (@list Constraint)) (n: Z) (BP0: Z) (retval: Z) (retval_
   **  (InequList remain n re )
 |--
   [| (l2 = (cons (x) (l3))) |] 
+  &&  [| (cur_coef <> 0) |] 
   &&  [| (cur <> 0) |] 
   &&  [| (l = (app (l1) (l2))) |] 
   &&  [| (eliminate_xn (Zto_nat ((num_pre - 1 ))) l1 bp ) |] 
@@ -1206,6 +1145,7 @@ Definition eliminate_partial_solve_wit_6 :=
 forall (num_pre: Z) (l: (@list Constraint)) (n: Z) (BP0: Z) (retval: Z) (retval_2: Z) (retval_3: Z) (cur: Z) (remain: Z) (lower: Z) (upper: Z) (up: (@list Constraint)) (lo: (@list Constraint)) (re: (@list Constraint)) (bp: BP) (l1: (@list Constraint)) (l2: (@list Constraint)) (cur_next: Z) (cur_coef: Z) (x: Constraint) (l3: (@list Constraint)) ,
   [| ((coef_Znth (num_pre) (x) (0)) <> 0) |] 
   &&  [| (l2 = (cons (x) (l3))) |] 
+  &&  [| (cur_coef <> 0) |] 
   &&  [| (cur <> 0) |] 
   &&  [| (l = (app (l1) (l2))) |] 
   &&  [| (eliminate_xn (Zto_nat ((num_pre - 1 ))) l1 bp ) |] 
@@ -1234,6 +1174,7 @@ forall (num_pre: Z) (l: (@list Constraint)) (n: Z) (BP0: Z) (retval: Z) (retval_
 |--
   [| ((coef_Znth (num_pre) (x) (0)) <> 0) |] 
   &&  [| (l2 = (cons (x) (l3))) |] 
+  &&  [| (cur_coef <> 0) |] 
   &&  [| (cur <> 0) |] 
   &&  [| (l = (app (l1) (l2))) |] 
   &&  [| (eliminate_xn (Zto_nat ((num_pre - 1 ))) l1 bp ) |] 
@@ -1268,7 +1209,8 @@ forall (n: Z) (l2: (@list Constraint)) (cur: Z) ,
   &&  (InequList cur n l2 )
 |--
   EX (cur_next: Z)  (cur_coef: Z)  (x: Constraint)  (l3: (@list Constraint)) ,
-  [| (l2 = (cons (x) (l3))) |]
+  [| (l2 = (cons (x) (l3))) |] 
+  &&  [| (cur_coef <> 0) |]
   &&  ((&((cur)  # "InequList" ->ₛ "coef")) # Ptr  |-> cur_coef)
   **  (coef_array cur_coef n x )
   **  ((&((cur)  # "InequList" ->ₛ "next")) # Ptr  |-> cur_next)
@@ -1282,6 +1224,8 @@ forall (cur_num_pre: Z) (num_pre: Z) (r2_pre: Z) (r1_pre: Z) (c2: Constraint) (c
   [| (0 <= cur_num_pre) |] 
   &&  [| (cur_num_pre < (num_pre + 1 )) |] 
   &&  [| ((num_pre + 1 ) <= INT_MAX) |] 
+  &&  [| (r1_pre <> 0) |] 
+  &&  [| (r2_pre <> 0) |] 
   &&  [| ((coef_Znth (cur_num_pre) (c1) (0)) > 0) |] 
   &&  [| ((coef_Znth (cur_num_pre) (c1) (0)) <= INT_MAX) |] 
   &&  [| ((coef_Znth (cur_num_pre) (c2) (0)) < 0) |] 
@@ -1304,6 +1248,8 @@ forall (cur_num_pre: Z) (num_pre: Z) (r2_pre: Z) (r1_pre: Z) (c2: Constraint) (c
   &&  [| (0 <= cur_num_pre) |] 
   &&  [| (cur_num_pre < (num_pre + 1 )) |] 
   &&  [| ((num_pre + 1 ) <= INT_MAX) |] 
+  &&  [| (r1_pre <> 0) |] 
+  &&  [| (r2_pre <> 0) |] 
   &&  [| ((coef_Znth (cur_num_pre) (c1) (0)) > 0) |] 
   &&  [| ((coef_Znth (cur_num_pre) (c1) (0)) <= INT_MAX) |] 
   &&  [| ((coef_Znth (cur_num_pre) (c2) (0)) < 0) |] 
@@ -1329,6 +1275,8 @@ forall (cur_num_pre: Z) (num_pre: Z) (r2_pre: Z) (r1_pre: Z) (c2: Constraint) (c
   &&  [| (0 <= cur_num_pre) |] 
   &&  [| (cur_num_pre < (num_pre + 1 )) |] 
   &&  [| ((num_pre + 1 ) <= INT_MAX) |] 
+  &&  [| (r1_pre <> 0) |] 
+  &&  [| (r2_pre <> 0) |] 
   &&  [| ((coef_Znth (cur_num_pre) (c1) (0)) > 0) |] 
   &&  [| ((coef_Znth (cur_num_pre) (c1) (0)) <= INT_MAX) |] 
   &&  [| ((coef_Znth (cur_num_pre) (c2) (0)) < 0) |] 
@@ -1355,6 +1303,8 @@ forall (cur_num_pre: Z) (num_pre: Z) (r2_pre: Z) (r1_pre: Z) (c2: Constraint) (c
   &&  [| (0 <= cur_num_pre) |] 
   &&  [| (cur_num_pre < (num_pre + 1 )) |] 
   &&  [| ((num_pre + 1 ) <= INT_MAX) |] 
+  &&  [| (r1_pre <> 0) |] 
+  &&  [| (r2_pre <> 0) |] 
   &&  [| ((coef_Znth (cur_num_pre) (c1) (0)) > 0) |] 
   &&  [| ((coef_Znth (cur_num_pre) (c1) (0)) <= INT_MAX) |] 
   &&  [| ((coef_Znth (cur_num_pre) (c2) (0)) < 0) |] 
@@ -1385,6 +1335,8 @@ forall (cur_num_pre: Z) (num_pre: Z) (r2_pre: Z) (r1_pre: Z) (c2: Constraint) (c
   &&  [| (0 <= cur_num_pre) |] 
   &&  [| (cur_num_pre < (num_pre + 1 )) |] 
   &&  [| ((num_pre + 1 ) <= INT_MAX) |] 
+  &&  [| (r1_pre <> 0) |] 
+  &&  [| (r2_pre <> 0) |] 
   &&  [| ((coef_Znth (cur_num_pre) (c1) (0)) > 0) |] 
   &&  [| ((coef_Znth (cur_num_pre) (c1) (0)) <= INT_MAX) |] 
   &&  [| ((coef_Znth (cur_num_pre) (c2) (0)) < 0) |] 
@@ -1415,6 +1367,8 @@ forall (cur_num_pre: Z) (num_pre: Z) (r2_pre: Z) (r1_pre: Z) (c2: Constraint) (c
   &&  [| (0 <= cur_num_pre) |] 
   &&  [| (cur_num_pre < (num_pre + 1 )) |] 
   &&  [| ((num_pre + 1 ) <= INT_MAX) |] 
+  &&  [| (r1_pre <> 0) |] 
+  &&  [| (r2_pre <> 0) |] 
   &&  [| ((coef_Znth (cur_num_pre) (c1) (0)) > 0) |] 
   &&  [| ((coef_Znth (cur_num_pre) (c1) (0)) <= INT_MAX) |] 
   &&  [| ((coef_Znth (cur_num_pre) (c2) (0)) < 0) |] 
@@ -1445,6 +1399,8 @@ forall (cur_num_pre: Z) (num_pre: Z) (r2_pre: Z) (r1_pre: Z) (c2: Constraint) (c
   &&  [| (0 <= cur_num_pre) |] 
   &&  [| (cur_num_pre < (num_pre + 1 )) |] 
   &&  [| ((num_pre + 1 ) <= INT_MAX) |] 
+  &&  [| (r1_pre <> 0) |] 
+  &&  [| (r2_pre <> 0) |] 
   &&  [| ((coef_Znth (cur_num_pre) (c1) (0)) > 0) |] 
   &&  [| ((coef_Znth (cur_num_pre) (c1) (0)) <= INT_MAX) |] 
   &&  [| ((coef_Znth (cur_num_pre) (c2) (0)) < 0) |] 
@@ -1474,6 +1430,8 @@ forall (cur_num_pre: Z) (num_pre: Z) (r2_pre: Z) (r1_pre: Z) (c2: Constraint) (c
   &&  [| (0 <= cur_num_pre) |] 
   &&  [| (cur_num_pre < (num_pre + 1 )) |] 
   &&  [| ((num_pre + 1 ) <= INT_MAX) |] 
+  &&  [| (r1_pre <> 0) |] 
+  &&  [| (r2_pre <> 0) |] 
   &&  [| ((coef_Znth (cur_num_pre) (c1) (0)) > 0) |] 
   &&  [| ((coef_Znth (cur_num_pre) (c1) (0)) <= INT_MAX) |] 
   &&  [| ((coef_Znth (cur_num_pre) (c2) (0)) < 0) |] 
@@ -1504,6 +1462,8 @@ forall (cur_num_pre: Z) (num_pre: Z) (r2_pre: Z) (r1_pre: Z) (c2: Constraint) (c
   &&  [| (0 <= cur_num_pre) |] 
   &&  [| (cur_num_pre < (num_pre + 1 )) |] 
   &&  [| ((num_pre + 1 ) <= INT_MAX) |] 
+  &&  [| (r1_pre <> 0) |] 
+  &&  [| (r2_pre <> 0) |] 
   &&  [| ((coef_Znth (cur_num_pre) (c1) (0)) > 0) |] 
   &&  [| ((coef_Znth (cur_num_pre) (c1) (0)) <= INT_MAX) |] 
   &&  [| ((coef_Znth (cur_num_pre) (c2) (0)) < 0) |] 
@@ -1534,6 +1494,8 @@ forall (cur_num_pre: Z) (num_pre: Z) (r2_pre: Z) (r1_pre: Z) (c2: Constraint) (c
   &&  [| (0 <= cur_num_pre) |] 
   &&  [| (cur_num_pre < (num_pre + 1 )) |] 
   &&  [| ((num_pre + 1 ) <= INT_MAX) |] 
+  &&  [| (r1_pre <> 0) |] 
+  &&  [| (r2_pre <> 0) |] 
   &&  [| ((coef_Znth (cur_num_pre) (c1) (0)) > 0) |] 
   &&  [| ((coef_Znth (cur_num_pre) (c1) (0)) <= INT_MAX) |] 
   &&  [| ((coef_Znth (cur_num_pre) (c2) (0)) < 0) |] 
@@ -1564,6 +1526,8 @@ forall (cur_num_pre: Z) (num_pre: Z) (r2_pre: Z) (r1_pre: Z) (c2: Constraint) (c
   &&  [| (0 <= cur_num_pre) |] 
   &&  [| (cur_num_pre < (num_pre + 1 )) |] 
   &&  [| ((num_pre + 1 ) <= INT_MAX) |] 
+  &&  [| (r1_pre <> 0) |] 
+  &&  [| (r2_pre <> 0) |] 
   &&  [| ((coef_Znth (cur_num_pre) (c1) (0)) > 0) |] 
   &&  [| ((coef_Znth (cur_num_pre) (c1) (0)) <= INT_MAX) |] 
   &&  [| ((coef_Znth (cur_num_pre) (c2) (0)) < 0) |] 
@@ -1594,6 +1558,8 @@ forall (cur_num_pre: Z) (num_pre: Z) (r2_pre: Z) (r1_pre: Z) (c2: Constraint) (c
   &&  [| (0 <= cur_num_pre) |] 
   &&  [| (cur_num_pre < (num_pre + 1 )) |] 
   &&  [| ((num_pre + 1 ) <= INT_MAX) |] 
+  &&  [| (r1_pre <> 0) |] 
+  &&  [| (r2_pre <> 0) |] 
   &&  [| ((coef_Znth (cur_num_pre) (c1) (0)) > 0) |] 
   &&  [| ((coef_Znth (cur_num_pre) (c1) (0)) <= INT_MAX) |] 
   &&  [| ((coef_Znth (cur_num_pre) (c2) (0)) < 0) |] 
@@ -1623,6 +1589,8 @@ forall (cur_num_pre: Z) (num_pre: Z) (r2_pre: Z) (r1_pre: Z) (c2: Constraint) (c
   &&  [| (0 <= cur_num_pre) |] 
   &&  [| (cur_num_pre < (num_pre + 1 )) |] 
   &&  [| ((num_pre + 1 ) <= INT_MAX) |] 
+  &&  [| (r1_pre <> 0) |] 
+  &&  [| (r2_pre <> 0) |] 
   &&  [| ((coef_Znth (cur_num_pre) (c1) (0)) > 0) |] 
   &&  [| ((coef_Znth (cur_num_pre) (c1) (0)) <= INT_MAX) |] 
   &&  [| ((coef_Znth (cur_num_pre) (c2) (0)) < 0) |] 
@@ -1653,6 +1621,8 @@ forall (cur_num_pre: Z) (num_pre: Z) (r2_pre: Z) (r1_pre: Z) (c2: Constraint) (c
   &&  [| (0 <= cur_num_pre) |] 
   &&  [| (cur_num_pre < (num_pre + 1 )) |] 
   &&  [| ((num_pre + 1 ) <= INT_MAX) |] 
+  &&  [| (r1_pre <> 0) |] 
+  &&  [| (r2_pre <> 0) |] 
   &&  [| ((coef_Znth (cur_num_pre) (c1) (0)) > 0) |] 
   &&  [| ((coef_Znth (cur_num_pre) (c1) (0)) <= INT_MAX) |] 
   &&  [| ((coef_Znth (cur_num_pre) (c2) (0)) < 0) |] 
@@ -1684,6 +1654,8 @@ forall (cur_num_pre: Z) (num_pre: Z) (r2_pre: Z) (r1_pre: Z) (c2: Constraint) (c
   &&  [| (0 <= cur_num_pre) |] 
   &&  [| (cur_num_pre < (num_pre + 1 )) |] 
   &&  [| ((num_pre + 1 ) <= INT_MAX) |] 
+  &&  [| (r1_pre <> 0) |] 
+  &&  [| (r2_pre <> 0) |] 
   &&  [| ((coef_Znth (cur_num_pre) (c1) (0)) > 0) |] 
   &&  [| ((coef_Znth (cur_num_pre) (c1) (0)) <= INT_MAX) |] 
   &&  [| ((coef_Znth (cur_num_pre) (c2) (0)) < 0) |] 
@@ -1727,6 +1699,8 @@ forall (cur_num_pre: Z) (num_pre: Z) (r2_pre: Z) (r1_pre: Z) (c2: Constraint) (c
   &&  [| (0 <= cur_num_pre) |] 
   &&  [| (cur_num_pre < (num_pre + 1 )) |] 
   &&  [| ((num_pre + 1 ) <= INT_MAX) |] 
+  &&  [| (r1_pre <> 0) |] 
+  &&  [| (r2_pre <> 0) |] 
   &&  [| ((coef_Znth (cur_num_pre) (c1) (0)) > 0) |] 
   &&  [| ((coef_Znth (cur_num_pre) (c1) (0)) <= INT_MAX) |] 
   &&  [| ((coef_Znth (cur_num_pre) (c2) (0)) < 0) |] 
@@ -1771,6 +1745,8 @@ forall (cur_num_pre: Z) (num_pre: Z) (r2_pre: Z) (r1_pre: Z) (c2: Constraint) (c
   &&  [| (0 <= cur_num_pre) |] 
   &&  [| (cur_num_pre < (num_pre + 1 )) |] 
   &&  [| ((num_pre + 1 ) <= INT_MAX) |] 
+  &&  [| (r1_pre <> 0) |] 
+  &&  [| (r2_pre <> 0) |] 
   &&  [| ((coef_Znth (cur_num_pre) (c1) (0)) > 0) |] 
   &&  [| ((coef_Znth (cur_num_pre) (c1) (0)) <= INT_MAX) |] 
   &&  [| ((coef_Znth (cur_num_pre) (c2) (0)) < 0) |] 
@@ -1816,6 +1792,8 @@ forall (cur_num_pre: Z) (num_pre: Z) (r2_pre: Z) (r1_pre: Z) (c2: Constraint) (c
   &&  [| (0 <= cur_num_pre) |] 
   &&  [| (cur_num_pre < (num_pre + 1 )) |] 
   &&  [| ((num_pre + 1 ) <= INT_MAX) |] 
+  &&  [| (r1_pre <> 0) |] 
+  &&  [| (r2_pre <> 0) |] 
   &&  [| ((coef_Znth (cur_num_pre) (c1) (0)) > 0) |] 
   &&  [| ((coef_Znth (cur_num_pre) (c1) (0)) <= INT_MAX) |] 
   &&  [| ((coef_Znth (cur_num_pre) (c2) (0)) < 0) |] 
@@ -1862,6 +1840,8 @@ forall (cur_num_pre: Z) (num_pre: Z) (r2_pre: Z) (r1_pre: Z) (c2: Constraint) (c
   &&  [| (0 <= cur_num_pre) |] 
   &&  [| (cur_num_pre < (num_pre + 1 )) |] 
   &&  [| ((num_pre + 1 ) <= INT_MAX) |] 
+  &&  [| (r1_pre <> 0) |] 
+  &&  [| (r2_pre <> 0) |] 
   &&  [| ((coef_Znth (cur_num_pre) (c1) (0)) > 0) |] 
   &&  [| ((coef_Znth (cur_num_pre) (c1) (0)) <= INT_MAX) |] 
   &&  [| ((coef_Znth (cur_num_pre) (c2) (0)) < 0) |] 
@@ -1908,6 +1888,8 @@ forall (cur_num_pre: Z) (num_pre: Z) (r2_pre: Z) (r1_pre: Z) (c2: Constraint) (c
   &&  [| (0 <= cur_num_pre) |] 
   &&  [| (cur_num_pre < (num_pre + 1 )) |] 
   &&  [| ((num_pre + 1 ) <= INT_MAX) |] 
+  &&  [| (r1_pre <> 0) |] 
+  &&  [| (r2_pre <> 0) |] 
   &&  [| ((coef_Znth (cur_num_pre) (c1) (0)) > 0) |] 
   &&  [| ((coef_Znth (cur_num_pre) (c1) (0)) <= INT_MAX) |] 
   &&  [| ((coef_Znth (cur_num_pre) (c2) (0)) < 0) |] 
@@ -1950,6 +1932,8 @@ forall (cur_num_pre: Z) (num_pre: Z) (r2_pre: Z) (r1_pre: Z) (c2: Constraint) (c
   &&  [| (0 <= cur_num_pre) |] 
   &&  [| (cur_num_pre < (num_pre + 1 )) |] 
   &&  [| ((num_pre + 1 ) <= INT_MAX) |] 
+  &&  [| (r1_pre <> 0) |] 
+  &&  [| (r2_pre <> 0) |] 
   &&  [| ((coef_Znth (cur_num_pre) (c1) (0)) > 0) |] 
   &&  [| ((coef_Znth (cur_num_pre) (c1) (0)) <= INT_MAX) |] 
   &&  [| ((coef_Znth (cur_num_pre) (c2) (0)) < 0) |] 
@@ -1993,6 +1977,8 @@ forall (cur_num_pre: Z) (num_pre: Z) (r2_pre: Z) (r1_pre: Z) (c2: Constraint) (c
   &&  [| (0 <= cur_num_pre) |] 
   &&  [| (cur_num_pre < (num_pre + 1 )) |] 
   &&  [| ((num_pre + 1 ) <= INT_MAX) |] 
+  &&  [| (r1_pre <> 0) |] 
+  &&  [| (r2_pre <> 0) |] 
   &&  [| ((coef_Znth (cur_num_pre) (c1) (0)) > 0) |] 
   &&  [| ((coef_Znth (cur_num_pre) (c1) (0)) <= INT_MAX) |] 
   &&  [| ((coef_Znth (cur_num_pre) (c2) (0)) < 0) |] 
@@ -2038,6 +2024,8 @@ forall (cur_num_pre: Z) (num_pre: Z) (r2_pre: Z) (r1_pre: Z) (c2: Constraint) (c
   &&  [| (0 <= cur_num_pre) |] 
   &&  [| (cur_num_pre < (num_pre + 1 )) |] 
   &&  [| ((num_pre + 1 ) <= INT_MAX) |] 
+  &&  [| (r1_pre <> 0) |] 
+  &&  [| (r2_pre <> 0) |] 
   &&  [| ((coef_Znth (cur_num_pre) (c1) (0)) > 0) |] 
   &&  [| ((coef_Znth (cur_num_pre) (c1) (0)) <= INT_MAX) |] 
   &&  [| ((coef_Znth (cur_num_pre) (c2) (0)) < 0) |] 
@@ -2094,6 +2082,8 @@ forall (cur_num_pre: Z) (num_pre: Z) (r2_pre: Z) (r1_pre: Z) (c2: Constraint) (c
   &&  [| (0 <= cur_num_pre) |] 
   &&  [| (cur_num_pre < (num_pre + 1 )) |] 
   &&  [| ((num_pre + 1 ) <= INT_MAX) |] 
+  &&  [| (r1_pre <> 0) |] 
+  &&  [| (r2_pre <> 0) |] 
   &&  [| ((coef_Znth (cur_num_pre) (c1) (0)) > 0) |] 
   &&  [| ((coef_Znth (cur_num_pre) (c1) (0)) <= INT_MAX) |] 
   &&  [| ((coef_Znth (cur_num_pre) (c2) (0)) < 0) |] 
@@ -2151,6 +2141,8 @@ forall (cur_num_pre: Z) (num_pre: Z) (r2_pre: Z) (r1_pre: Z) (c2: Constraint) (c
   &&  [| (0 <= cur_num_pre) |] 
   &&  [| (cur_num_pre < (num_pre + 1 )) |] 
   &&  [| ((num_pre + 1 ) <= INT_MAX) |] 
+  &&  [| (r1_pre <> 0) |] 
+  &&  [| (r2_pre <> 0) |] 
   &&  [| ((coef_Znth (cur_num_pre) (c1) (0)) > 0) |] 
   &&  [| ((coef_Znth (cur_num_pre) (c1) (0)) <= INT_MAX) |] 
   &&  [| ((coef_Znth (cur_num_pre) (c2) (0)) < 0) |] 
@@ -2211,6 +2203,8 @@ forall (cur_num_pre: Z) (num_pre: Z) (r2_pre: Z) (r1_pre: Z) (c2: Constraint) (c
   &&  [| (0 <= cur_num_pre) |] 
   &&  [| (cur_num_pre < (num_pre + 1 )) |] 
   &&  [| ((num_pre + 1 ) <= INT_MAX) |] 
+  &&  [| (r1_pre <> 0) |] 
+  &&  [| (r2_pre <> 0) |] 
   &&  [| ((coef_Znth (cur_num_pre) (c1) (0)) > 0) |] 
   &&  [| ((coef_Znth (cur_num_pre) (c1) (0)) <= INT_MAX) |] 
   &&  [| ((coef_Znth (cur_num_pre) (c2) (0)) < 0) |] 
@@ -2272,6 +2266,8 @@ forall (cur_num_pre: Z) (num_pre: Z) (r2_pre: Z) (r1_pre: Z) (c2: Constraint) (c
   &&  [| (0 <= cur_num_pre) |] 
   &&  [| (cur_num_pre < (num_pre + 1 )) |] 
   &&  [| ((num_pre + 1 ) <= INT_MAX) |] 
+  &&  [| (r1_pre <> 0) |] 
+  &&  [| (r2_pre <> 0) |] 
   &&  [| ((coef_Znth (cur_num_pre) (c1) (0)) > 0) |] 
   &&  [| ((coef_Znth (cur_num_pre) (c1) (0)) <= INT_MAX) |] 
   &&  [| ((coef_Znth (cur_num_pre) (c2) (0)) < 0) |] 
@@ -2331,6 +2327,8 @@ forall (cur_num_pre: Z) (num_pre: Z) (r2_pre: Z) (r1_pre: Z) (c2: Constraint) (c
   &&  [| (0 <= cur_num_pre) |] 
   &&  [| (cur_num_pre < (num_pre + 1 )) |] 
   &&  [| ((num_pre + 1 ) <= INT_MAX) |] 
+  &&  [| (r1_pre <> 0) |] 
+  &&  [| (r2_pre <> 0) |] 
   &&  [| ((coef_Znth (cur_num_pre) (c1) (0)) > 0) |] 
   &&  [| ((coef_Znth (cur_num_pre) (c1) (0)) <= INT_MAX) |] 
   &&  [| ((coef_Znth (cur_num_pre) (c2) (0)) < 0) |] 
@@ -2392,6 +2390,8 @@ forall (cur_num_pre: Z) (num_pre: Z) (r2_pre: Z) (r1_pre: Z) (c2: Constraint) (c
   &&  [| (0 <= cur_num_pre) |] 
   &&  [| (cur_num_pre < (num_pre + 1 )) |] 
   &&  [| ((num_pre + 1 ) <= INT_MAX) |] 
+  &&  [| (r1_pre <> 0) |] 
+  &&  [| (r2_pre <> 0) |] 
   &&  [| ((coef_Znth (cur_num_pre) (c1) (0)) > 0) |] 
   &&  [| ((coef_Znth (cur_num_pre) (c1) (0)) <= INT_MAX) |] 
   &&  [| ((coef_Znth (cur_num_pre) (c2) (0)) < 0) |] 
@@ -2454,6 +2454,8 @@ forall (cur_num_pre: Z) (num_pre: Z) (r2_pre: Z) (r1_pre: Z) (c2: Constraint) (c
   &&  [| (0 <= cur_num_pre) |] 
   &&  [| (cur_num_pre < (num_pre + 1 )) |] 
   &&  [| ((num_pre + 1 ) <= INT_MAX) |] 
+  &&  [| (r1_pre <> 0) |] 
+  &&  [| (r2_pre <> 0) |] 
   &&  [| ((coef_Znth (cur_num_pre) (c1) (0)) > 0) |] 
   &&  [| ((coef_Znth (cur_num_pre) (c1) (0)) <= INT_MAX) |] 
   &&  [| ((coef_Znth (cur_num_pre) (c2) (0)) < 0) |] 
@@ -2488,6 +2490,8 @@ forall (cur_num_pre: Z) (num_pre: Z) (r2_pre: Z) (r1_pre: Z) (c2: Constraint) (c
   &&  [| (0 <= cur_num_pre) |] 
   &&  [| (cur_num_pre < (num_pre + 1 )) |] 
   &&  [| ((num_pre + 1 ) <= INT_MAX) |] 
+  &&  [| (r1_pre <> 0) |] 
+  &&  [| (r2_pre <> 0) |] 
   &&  [| ((coef_Znth (cur_num_pre) (c1) (0)) > 0) |] 
   &&  [| ((coef_Znth (cur_num_pre) (c1) (0)) <= INT_MAX) |] 
   &&  [| ((coef_Znth (cur_num_pre) (c2) (0)) < 0) |] 
@@ -2509,6 +2513,8 @@ forall (cur_num_pre: Z) (num_pre: Z) (r2_pre: Z) (r1_pre: Z) (c2: Constraint) (c
   &&  [| (0 <= cur_num_pre) |] 
   &&  [| (cur_num_pre < (num_pre + 1 )) |] 
   &&  [| ((num_pre + 1 ) <= INT_MAX) |] 
+  &&  [| (r1_pre <> 0) |] 
+  &&  [| (r2_pre <> 0) |] 
   &&  [| ((coef_Znth (cur_num_pre) (c1) (0)) > 0) |] 
   &&  [| ((coef_Znth (cur_num_pre) (c1) (0)) <= INT_MAX) |] 
   &&  [| ((coef_Znth (cur_num_pre) (c2) (0)) < 0) |] 
@@ -2538,6 +2544,8 @@ forall (cur_num_pre: Z) (num_pre: Z) (r2_pre: Z) (r1_pre: Z) (c2: Constraint) (c
   &&  [| (0 <= cur_num_pre) |] 
   &&  [| (cur_num_pre < (num_pre + 1 )) |] 
   &&  [| ((num_pre + 1 ) <= INT_MAX) |] 
+  &&  [| (r1_pre <> 0) |] 
+  &&  [| (r2_pre <> 0) |] 
   &&  [| ((coef_Znth (cur_num_pre) (c1) (0)) > 0) |] 
   &&  [| ((coef_Znth (cur_num_pre) (c1) (0)) <= INT_MAX) |] 
   &&  [| ((coef_Znth (cur_num_pre) (c2) (0)) < 0) |] 
@@ -2559,6 +2567,8 @@ forall (cur_num_pre: Z) (num_pre: Z) (r2_pre: Z) (r1_pre: Z) (c2: Constraint) (c
   &&  [| (0 <= cur_num_pre) |] 
   &&  [| (cur_num_pre < (num_pre + 1 )) |] 
   &&  [| ((num_pre + 1 ) <= INT_MAX) |] 
+  &&  [| (r1_pre <> 0) |] 
+  &&  [| (r2_pre <> 0) |] 
   &&  [| ((coef_Znth (cur_num_pre) (c1) (0)) > 0) |] 
   &&  [| ((coef_Znth (cur_num_pre) (c1) (0)) <= INT_MAX) |] 
   &&  [| ((coef_Znth (cur_num_pre) (c2) (0)) < 0) |] 
@@ -2586,6 +2596,8 @@ forall (cur_num_pre: Z) (num_pre: Z) (r2_pre: Z) (r1_pre: Z) (c2: Constraint) (c
   &&  [| (0 <= cur_num_pre) |] 
   &&  [| (cur_num_pre < (num_pre + 1 )) |] 
   &&  [| ((num_pre + 1 ) <= INT_MAX) |] 
+  &&  [| (r1_pre <> 0) |] 
+  &&  [| (r2_pre <> 0) |] 
   &&  [| ((coef_Znth (cur_num_pre) (c1) (0)) > 0) |] 
   &&  [| ((coef_Znth (cur_num_pre) (c1) (0)) <= INT_MAX) |] 
   &&  [| ((coef_Znth (cur_num_pre) (c2) (0)) < 0) |] 
@@ -2621,6 +2633,8 @@ forall (cur_num_pre: Z) (num_pre: Z) (r2_pre: Z) (r1_pre: Z) (c2: Constraint) (c
   &&  [| (0 <= cur_num_pre) |] 
   &&  [| (cur_num_pre < (num_pre + 1 )) |] 
   &&  [| ((num_pre + 1 ) <= INT_MAX) |] 
+  &&  [| (r1_pre <> 0) |] 
+  &&  [| (r2_pre <> 0) |] 
   &&  [| ((coef_Znth (cur_num_pre) (c1) (0)) > 0) |] 
   &&  [| ((coef_Znth (cur_num_pre) (c1) (0)) <= INT_MAX) |] 
   &&  [| ((coef_Znth (cur_num_pre) (c2) (0)) < 0) |] 
@@ -2663,6 +2677,8 @@ forall (cur_num_pre: Z) (num_pre: Z) (r2_pre: Z) (r1_pre: Z) (c2: Constraint) (c
   &&  [| (0 <= cur_num_pre) |] 
   &&  [| (cur_num_pre < (num_pre + 1 )) |] 
   &&  [| ((num_pre + 1 ) <= INT_MAX) |] 
+  &&  [| (r1_pre <> 0) |] 
+  &&  [| (r2_pre <> 0) |] 
   &&  [| ((coef_Znth (cur_num_pre) (c1) (0)) > 0) |] 
   &&  [| ((coef_Znth (cur_num_pre) (c1) (0)) <= INT_MAX) |] 
   &&  [| ((coef_Znth (cur_num_pre) (c2) (0)) < 0) |] 
@@ -2699,6 +2715,8 @@ forall (cur_num_pre: Z) (num_pre: Z) (r2_pre: Z) (r1_pre: Z) (c2: Constraint) (c
   &&  [| (0 <= cur_num_pre) |] 
   &&  [| (cur_num_pre < (num_pre + 1 )) |] 
   &&  [| ((num_pre + 1 ) <= INT_MAX) |] 
+  &&  [| (r1_pre <> 0) |] 
+  &&  [| (r2_pre <> 0) |] 
   &&  [| ((coef_Znth (cur_num_pre) (c1) (0)) > 0) |] 
   &&  [| ((coef_Znth (cur_num_pre) (c1) (0)) <= INT_MAX) |] 
   &&  [| ((coef_Znth (cur_num_pre) (c2) (0)) < 0) |] 
@@ -2739,6 +2757,8 @@ forall (cur_num_pre: Z) (num_pre: Z) (r2_pre: Z) (r1_pre: Z) (c2: Constraint) (c
   &&  [| (0 <= cur_num_pre) |] 
   &&  [| (cur_num_pre < (num_pre + 1 )) |] 
   &&  [| ((num_pre + 1 ) <= INT_MAX) |] 
+  &&  [| (r1_pre <> 0) |] 
+  &&  [| (r2_pre <> 0) |] 
   &&  [| ((coef_Znth (cur_num_pre) (c1) (0)) > 0) |] 
   &&  [| ((coef_Znth (cur_num_pre) (c1) (0)) <= INT_MAX) |] 
   &&  [| ((coef_Znth (cur_num_pre) (c2) (0)) < 0) |] 
@@ -2778,6 +2798,8 @@ forall (cur_num_pre: Z) (num_pre: Z) (r2_pre: Z) (r1_pre: Z) (c2: Constraint) (c
   &&  [| (0 <= cur_num_pre) |] 
   &&  [| (cur_num_pre < (num_pre + 1 )) |] 
   &&  [| ((num_pre + 1 ) <= INT_MAX) |] 
+  &&  [| (r1_pre <> 0) |] 
+  &&  [| (r2_pre <> 0) |] 
   &&  [| ((coef_Znth (cur_num_pre) (c1) (0)) > 0) |] 
   &&  [| ((coef_Znth (cur_num_pre) (c1) (0)) <= INT_MAX) |] 
   &&  [| ((coef_Znth (cur_num_pre) (c2) (0)) < 0) |] 
@@ -2816,6 +2838,8 @@ forall (cur_num_pre: Z) (num_pre: Z) (r2_pre: Z) (r1_pre: Z) (c2: Constraint) (c
   &&  [| (0 <= cur_num_pre) |] 
   &&  [| (cur_num_pre < (num_pre + 1 )) |] 
   &&  [| ((num_pre + 1 ) <= INT_MAX) |] 
+  &&  [| (r1_pre <> 0) |] 
+  &&  [| (r2_pre <> 0) |] 
   &&  [| ((coef_Znth (cur_num_pre) (c1) (0)) > 0) |] 
   &&  [| ((coef_Znth (cur_num_pre) (c1) (0)) <= INT_MAX) |] 
   &&  [| ((coef_Znth (cur_num_pre) (c2) (0)) < 0) |] 
@@ -2857,6 +2881,8 @@ forall (cur_num_pre: Z) (num_pre: Z) (r2_pre: Z) (r1_pre: Z) (c2: Constraint) (c
   &&  [| (0 <= cur_num_pre) |] 
   &&  [| (cur_num_pre < (num_pre + 1 )) |] 
   &&  [| ((num_pre + 1 ) <= INT_MAX) |] 
+  &&  [| (r1_pre <> 0) |] 
+  &&  [| (r2_pre <> 0) |] 
   &&  [| ((coef_Znth (cur_num_pre) (c1) (0)) > 0) |] 
   &&  [| ((coef_Znth (cur_num_pre) (c1) (0)) <= INT_MAX) |] 
   &&  [| ((coef_Znth (cur_num_pre) (c2) (0)) < 0) |] 
@@ -2897,6 +2923,8 @@ forall (cur_num_pre: Z) (num_pre: Z) (r2_pre: Z) (r1_pre: Z) (c2: Constraint) (c
   &&  [| (0 <= cur_num_pre) |] 
   &&  [| (cur_num_pre < (num_pre + 1 )) |] 
   &&  [| ((num_pre + 1 ) <= INT_MAX) |] 
+  &&  [| (r1_pre <> 0) |] 
+  &&  [| (r2_pre <> 0) |] 
   &&  [| ((coef_Znth (cur_num_pre) (c1) (0)) > 0) |] 
   &&  [| ((coef_Znth (cur_num_pre) (c1) (0)) <= INT_MAX) |] 
   &&  [| ((coef_Znth (cur_num_pre) (c2) (0)) < 0) |] 
@@ -2946,6 +2974,8 @@ forall (cur_num_pre: Z) (num_pre: Z) (r2_pre: Z) (r1_pre: Z) (c2: Constraint) (c
   &&  [| (0 <= cur_num_pre) |] 
   &&  [| (cur_num_pre < (num_pre + 1 )) |] 
   &&  [| ((num_pre + 1 ) <= INT_MAX) |] 
+  &&  [| (r1_pre <> 0) |] 
+  &&  [| (r2_pre <> 0) |] 
   &&  [| ((coef_Znth (cur_num_pre) (c1) (0)) > 0) |] 
   &&  [| ((coef_Znth (cur_num_pre) (c1) (0)) <= INT_MAX) |] 
   &&  [| ((coef_Znth (cur_num_pre) (c2) (0)) < 0) |] 
@@ -2972,6 +3002,8 @@ forall (cur_num_pre: Z) (num_pre: Z) (r2_pre: Z) (r1_pre: Z) (c2: Constraint) (c
   [| (0 <= cur_num_pre) |] 
   &&  [| (cur_num_pre < (num_pre + 1 )) |] 
   &&  [| ((num_pre + 1 ) <= INT_MAX) |] 
+  &&  [| (r1_pre <> 0) |] 
+  &&  [| (r2_pre <> 0) |] 
   &&  [| ((coef_Znth (cur_num_pre) (c1) (0)) > 0) |] 
   &&  [| ((coef_Znth (cur_num_pre) (c1) (0)) <= INT_MAX) |] 
   &&  [| ((coef_Znth (cur_num_pre) (c2) (0)) < 0) |] 
@@ -2982,6 +3014,8 @@ forall (cur_num_pre: Z) (num_pre: Z) (r2_pre: Z) (r1_pre: Z) (c2: Constraint) (c
   [| (0 <= cur_num_pre) |] 
   &&  [| (cur_num_pre < (num_pre + 1 )) |] 
   &&  [| ((num_pre + 1 ) <= INT_MAX) |] 
+  &&  [| (r1_pre <> 0) |] 
+  &&  [| (r2_pre <> 0) |] 
   &&  [| ((coef_Znth (cur_num_pre) (c1) (0)) > 0) |] 
   &&  [| ((coef_Znth (cur_num_pre) (c1) (0)) <= INT_MAX) |] 
   &&  [| ((coef_Znth (cur_num_pre) (c2) (0)) < 0) |] 
@@ -2996,6 +3030,8 @@ forall (cur_num_pre: Z) (num_pre: Z) (r2_pre: Z) (r1_pre: Z) (c2: Constraint) (c
   [| (0 <= cur_num_pre) |] 
   &&  [| (cur_num_pre < (num_pre + 1 )) |] 
   &&  [| ((num_pre + 1 ) <= INT_MAX) |] 
+  &&  [| (r1_pre <> 0) |] 
+  &&  [| (r2_pre <> 0) |] 
   &&  [| ((coef_Znth (cur_num_pre) (c1) (0)) > 0) |] 
   &&  [| ((coef_Znth (cur_num_pre) (c1) (0)) <= INT_MAX) |] 
   &&  [| ((coef_Znth (cur_num_pre) (c2) (0)) < 0) |] 
@@ -3006,6 +3042,8 @@ forall (cur_num_pre: Z) (num_pre: Z) (r2_pre: Z) (r1_pre: Z) (c2: Constraint) (c
   [| (0 <= cur_num_pre) |] 
   &&  [| (cur_num_pre < (num_pre + 1 )) |] 
   &&  [| ((num_pre + 1 ) <= INT_MAX) |] 
+  &&  [| (r1_pre <> 0) |] 
+  &&  [| (r2_pre <> 0) |] 
   &&  [| ((coef_Znth (cur_num_pre) (c1) (0)) > 0) |] 
   &&  [| ((coef_Znth (cur_num_pre) (c1) (0)) <= INT_MAX) |] 
   &&  [| ((coef_Znth (cur_num_pre) (c2) (0)) < 0) |] 
@@ -3020,6 +3058,8 @@ forall (cur_num_pre: Z) (num_pre: Z) (r2_pre: Z) (r1_pre: Z) (c2: Constraint) (c
   [| (0 <= cur_num_pre) |] 
   &&  [| (cur_num_pre < (num_pre + 1 )) |] 
   &&  [| ((num_pre + 1 ) <= INT_MAX) |] 
+  &&  [| (r1_pre <> 0) |] 
+  &&  [| (r2_pre <> 0) |] 
   &&  [| ((coef_Znth (cur_num_pre) (c1) (0)) > 0) |] 
   &&  [| ((coef_Znth (cur_num_pre) (c1) (0)) <= INT_MAX) |] 
   &&  [| ((coef_Znth (cur_num_pre) (c2) (0)) < 0) |] 
@@ -3045,6 +3085,8 @@ forall (cur_num_pre: Z) (num_pre: Z) (r2_pre: Z) (r1_pre: Z) (c2: Constraint) (c
   [| (0 <= cur_num_pre) |] 
   &&  [| (cur_num_pre < (num_pre + 1 )) |] 
   &&  [| ((num_pre + 1 ) <= INT_MAX) |] 
+  &&  [| (r1_pre <> 0) |] 
+  &&  [| (r2_pre <> 0) |] 
   &&  [| ((coef_Znth (cur_num_pre) (c1) (0)) > 0) |] 
   &&  [| ((coef_Znth (cur_num_pre) (c1) (0)) <= INT_MAX) |] 
   &&  [| ((coef_Znth (cur_num_pre) (c2) (0)) < 0) |] 
@@ -3059,6 +3101,8 @@ forall (cur_num_pre: Z) (num_pre: Z) (r2_pre: Z) (r1_pre: Z) (c2: Constraint) (c
   &&  [| (0 <= cur_num_pre) |] 
   &&  [| (cur_num_pre < (num_pre + 1 )) |] 
   &&  [| ((num_pre + 1 ) <= INT_MAX) |] 
+  &&  [| (r1_pre <> 0) |] 
+  &&  [| (r2_pre <> 0) |] 
   &&  [| ((coef_Znth (cur_num_pre) (c1) (0)) > 0) |] 
   &&  [| ((coef_Znth (cur_num_pre) (c1) (0)) <= INT_MAX) |] 
   &&  [| ((coef_Znth (cur_num_pre) (c2) (0)) < 0) |] 
@@ -3086,6 +3130,8 @@ forall (cur_num_pre: Z) (num_pre: Z) (r2_pre: Z) (r1_pre: Z) (c2: Constraint) (c
   &&  [| (0 <= cur_num_pre) |] 
   &&  [| (cur_num_pre < (num_pre + 1 )) |] 
   &&  [| ((num_pre + 1 ) <= INT_MAX) |] 
+  &&  [| (r1_pre <> 0) |] 
+  &&  [| (r2_pre <> 0) |] 
   &&  [| ((coef_Znth (cur_num_pre) (c1) (0)) > 0) |] 
   &&  [| ((coef_Znth (cur_num_pre) (c1) (0)) <= INT_MAX) |] 
   &&  [| ((coef_Znth (cur_num_pre) (c2) (0)) < 0) |] 
@@ -3108,6 +3154,8 @@ forall (cur_num_pre: Z) (num_pre: Z) (r2_pre: Z) (r1_pre: Z) (c2: Constraint) (c
   &&  [| (0 <= cur_num_pre) |] 
   &&  [| (cur_num_pre < (num_pre + 1 )) |] 
   &&  [| ((num_pre + 1 ) <= INT_MAX) |] 
+  &&  [| (r1_pre <> 0) |] 
+  &&  [| (r2_pre <> 0) |] 
   &&  [| ((coef_Znth (cur_num_pre) (c1) (0)) > 0) |] 
   &&  [| ((coef_Znth (cur_num_pre) (c1) (0)) <= INT_MAX) |] 
   &&  [| ((coef_Znth (cur_num_pre) (c2) (0)) < 0) |] 
@@ -3135,6 +3183,8 @@ forall (cur_num_pre: Z) (num_pre: Z) (r2_pre: Z) (r1_pre: Z) (c2: Constraint) (c
   &&  [| (0 <= cur_num_pre) |] 
   &&  [| (cur_num_pre < (num_pre + 1 )) |] 
   &&  [| ((num_pre + 1 ) <= INT_MAX) |] 
+  &&  [| (r1_pre <> 0) |] 
+  &&  [| (r2_pre <> 0) |] 
   &&  [| ((coef_Znth (cur_num_pre) (c1) (0)) > 0) |] 
   &&  [| ((coef_Znth (cur_num_pre) (c1) (0)) <= INT_MAX) |] 
   &&  [| ((coef_Znth (cur_num_pre) (c2) (0)) < 0) |] 
@@ -3158,6 +3208,8 @@ forall (cur_num_pre: Z) (num_pre: Z) (r2_pre: Z) (r1_pre: Z) (c2: Constraint) (c
   &&  [| (0 <= cur_num_pre) |] 
   &&  [| (cur_num_pre < (num_pre + 1 )) |] 
   &&  [| ((num_pre + 1 ) <= INT_MAX) |] 
+  &&  [| (r1_pre <> 0) |] 
+  &&  [| (r2_pre <> 0) |] 
   &&  [| ((coef_Znth (cur_num_pre) (c1) (0)) > 0) |] 
   &&  [| ((coef_Znth (cur_num_pre) (c1) (0)) <= INT_MAX) |] 
   &&  [| ((coef_Znth (cur_num_pre) (c2) (0)) < 0) |] 
@@ -3186,6 +3238,8 @@ forall (cur_num_pre: Z) (num_pre: Z) (r2_pre: Z) (r1_pre: Z) (c2: Constraint) (c
   &&  [| (0 <= cur_num_pre) |] 
   &&  [| (cur_num_pre < (num_pre + 1 )) |] 
   &&  [| ((num_pre + 1 ) <= INT_MAX) |] 
+  &&  [| (r1_pre <> 0) |] 
+  &&  [| (r2_pre <> 0) |] 
   &&  [| ((coef_Znth (cur_num_pre) (c1) (0)) > 0) |] 
   &&  [| ((coef_Znth (cur_num_pre) (c1) (0)) <= INT_MAX) |] 
   &&  [| ((coef_Znth (cur_num_pre) (c2) (0)) < 0) |] 
@@ -3210,6 +3264,8 @@ forall (cur_num_pre: Z) (num_pre: Z) (r2_pre: Z) (r1_pre: Z) (c2: Constraint) (c
   &&  [| (0 <= cur_num_pre) |] 
   &&  [| (cur_num_pre < (num_pre + 1 )) |] 
   &&  [| ((num_pre + 1 ) <= INT_MAX) |] 
+  &&  [| (r1_pre <> 0) |] 
+  &&  [| (r2_pre <> 0) |] 
   &&  [| ((coef_Znth (cur_num_pre) (c1) (0)) > 0) |] 
   &&  [| ((coef_Znth (cur_num_pre) (c1) (0)) <= INT_MAX) |] 
   &&  [| ((coef_Znth (cur_num_pre) (c2) (0)) < 0) |] 
@@ -3239,6 +3295,8 @@ forall (cur_num_pre: Z) (num_pre: Z) (r2_pre: Z) (r1_pre: Z) (c2: Constraint) (c
   &&  [| (0 <= cur_num_pre) |] 
   &&  [| (cur_num_pre < (num_pre + 1 )) |] 
   &&  [| ((num_pre + 1 ) <= INT_MAX) |] 
+  &&  [| (r1_pre <> 0) |] 
+  &&  [| (r2_pre <> 0) |] 
   &&  [| ((coef_Znth (cur_num_pre) (c1) (0)) > 0) |] 
   &&  [| ((coef_Znth (cur_num_pre) (c1) (0)) <= INT_MAX) |] 
   &&  [| ((coef_Znth (cur_num_pre) (c2) (0)) < 0) |] 
@@ -3264,6 +3322,8 @@ forall (cur_num_pre: Z) (num_pre: Z) (r2_pre: Z) (r1_pre: Z) (c2: Constraint) (c
   &&  [| (0 <= cur_num_pre) |] 
   &&  [| (cur_num_pre < (num_pre + 1 )) |] 
   &&  [| ((num_pre + 1 ) <= INT_MAX) |] 
+  &&  [| (r1_pre <> 0) |] 
+  &&  [| (r2_pre <> 0) |] 
   &&  [| ((coef_Znth (cur_num_pre) (c1) (0)) > 0) |] 
   &&  [| ((coef_Znth (cur_num_pre) (c1) (0)) <= INT_MAX) |] 
   &&  [| ((coef_Znth (cur_num_pre) (c2) (0)) < 0) |] 
@@ -3290,6 +3350,8 @@ forall (cur_num_pre: Z) (num_pre: Z) (r2_pre: Z) (r1_pre: Z) (c2: Constraint) (c
   &&  [| (0 <= cur_num_pre) |] 
   &&  [| (cur_num_pre < (num_pre + 1 )) |] 
   &&  [| ((num_pre + 1 ) <= INT_MAX) |] 
+  &&  [| (r1_pre <> 0) |] 
+  &&  [| (r2_pre <> 0) |] 
   &&  [| ((coef_Znth (cur_num_pre) (c1) (0)) > 0) |] 
   &&  [| ((coef_Znth (cur_num_pre) (c1) (0)) <= INT_MAX) |] 
   &&  [| ((coef_Znth (cur_num_pre) (c2) (0)) < 0) |] 
@@ -3312,6 +3374,8 @@ forall (cur_num_pre: Z) (num_pre: Z) (r2_pre: Z) (r1_pre: Z) (c2: Constraint) (c
   &&  [| (0 <= cur_num_pre) |] 
   &&  [| (cur_num_pre < (num_pre + 1 )) |] 
   &&  [| ((num_pre + 1 ) <= INT_MAX) |] 
+  &&  [| (r1_pre <> 0) |] 
+  &&  [| (r2_pre <> 0) |] 
   &&  [| ((coef_Znth (cur_num_pre) (c1) (0)) > 0) |] 
   &&  [| ((coef_Znth (cur_num_pre) (c1) (0)) <= INT_MAX) |] 
   &&  [| ((coef_Znth (cur_num_pre) (c2) (0)) < 0) |] 
@@ -3349,6 +3413,8 @@ forall (cur_num_pre: Z) (num_pre: Z) (r2_pre: Z) (r1_pre: Z) (c2: Constraint) (c
   &&  [| (0 <= cur_num_pre) |] 
   &&  [| (cur_num_pre < (num_pre + 1 )) |] 
   &&  [| ((num_pre + 1 ) <= INT_MAX) |] 
+  &&  [| (r1_pre <> 0) |] 
+  &&  [| (r2_pre <> 0) |] 
   &&  [| ((coef_Znth (cur_num_pre) (c1) (0)) > 0) |] 
   &&  [| ((coef_Znth (cur_num_pre) (c1) (0)) <= INT_MAX) |] 
   &&  [| ((coef_Znth (cur_num_pre) (c2) (0)) < 0) |] 
@@ -3384,6 +3450,8 @@ forall (cur_num_pre: Z) (num_pre: Z) (r2_pre: Z) (r1_pre: Z) (c2: Constraint) (c
   &&  [| (0 <= cur_num_pre) |] 
   &&  [| (cur_num_pre < (num_pre + 1 )) |] 
   &&  [| ((num_pre + 1 ) <= INT_MAX) |] 
+  &&  [| (r1_pre <> 0) |] 
+  &&  [| (r2_pre <> 0) |] 
   &&  [| ((coef_Znth (cur_num_pre) (c1) (0)) > 0) |] 
   &&  [| ((coef_Znth (cur_num_pre) (c1) (0)) <= INT_MAX) |] 
   &&  [| ((coef_Znth (cur_num_pre) (c2) (0)) < 0) |] 
@@ -3423,6 +3491,8 @@ forall (cur_num_pre: Z) (num_pre: Z) (r2_pre: Z) (r1_pre: Z) (c2: Constraint) (c
   &&  [| (0 <= cur_num_pre) |] 
   &&  [| (cur_num_pre < (num_pre + 1 )) |] 
   &&  [| ((num_pre + 1 ) <= INT_MAX) |] 
+  &&  [| (r1_pre <> 0) |] 
+  &&  [| (r2_pre <> 0) |] 
   &&  [| ((coef_Znth (cur_num_pre) (c1) (0)) > 0) |] 
   &&  [| ((coef_Znth (cur_num_pre) (c1) (0)) <= INT_MAX) |] 
   &&  [| ((coef_Znth (cur_num_pre) (c2) (0)) < 0) |] 
@@ -3458,6 +3528,8 @@ forall (cur_num_pre: Z) (num_pre: Z) (r2_pre: Z) (r1_pre: Z) (c2: Constraint) (c
   &&  [| (0 <= cur_num_pre) |] 
   &&  [| (cur_num_pre < (num_pre + 1 )) |] 
   &&  [| ((num_pre + 1 ) <= INT_MAX) |] 
+  &&  [| (r1_pre <> 0) |] 
+  &&  [| (r2_pre <> 0) |] 
   &&  [| ((coef_Znth (cur_num_pre) (c1) (0)) > 0) |] 
   &&  [| ((coef_Znth (cur_num_pre) (c1) (0)) <= INT_MAX) |] 
   &&  [| ((coef_Znth (cur_num_pre) (c2) (0)) < 0) |] 
@@ -3497,6 +3569,8 @@ forall (cur_num_pre: Z) (num_pre: Z) (r2_pre: Z) (r1_pre: Z) (c2: Constraint) (c
   &&  [| (0 <= cur_num_pre) |] 
   &&  [| (cur_num_pre < (num_pre + 1 )) |] 
   &&  [| ((num_pre + 1 ) <= INT_MAX) |] 
+  &&  [| (r1_pre <> 0) |] 
+  &&  [| (r2_pre <> 0) |] 
   &&  [| ((coef_Znth (cur_num_pre) (c1) (0)) > 0) |] 
   &&  [| ((coef_Znth (cur_num_pre) (c1) (0)) <= INT_MAX) |] 
   &&  [| ((coef_Znth (cur_num_pre) (c2) (0)) < 0) |] 
@@ -3557,6 +3631,8 @@ forall (cur_num_pre: Z) (num_pre: Z) (r2_pre: Z) (r1_pre: Z) (c2: Constraint) (c
   &&  [| (0 <= cur_num_pre) |] 
   &&  [| (cur_num_pre < (num_pre + 1 )) |] 
   &&  [| ((num_pre + 1 ) <= INT_MAX) |] 
+  &&  [| (r1_pre <> 0) |] 
+  &&  [| (r2_pre <> 0) |] 
   &&  [| ((coef_Znth (cur_num_pre) (c1) (0)) > 0) |] 
   &&  [| ((coef_Znth (cur_num_pre) (c1) (0)) <= INT_MAX) |] 
   &&  [| ((coef_Znth (cur_num_pre) (c2) (0)) < 0) |] 
@@ -3596,6 +3672,8 @@ forall (cur_num_pre: Z) (num_pre: Z) (r2_pre: Z) (r1_pre: Z) (c2: Constraint) (c
   &&  [| (0 <= cur_num_pre) |] 
   &&  [| (cur_num_pre < (num_pre + 1 )) |] 
   &&  [| ((num_pre + 1 ) <= INT_MAX) |] 
+  &&  [| (r1_pre <> 0) |] 
+  &&  [| (r2_pre <> 0) |] 
   &&  [| ((coef_Znth (cur_num_pre) (c1) (0)) > 0) |] 
   &&  [| ((coef_Znth (cur_num_pre) (c1) (0)) <= INT_MAX) |] 
   &&  [| ((coef_Znth (cur_num_pre) (c2) (0)) < 0) |] 
@@ -3638,6 +3716,8 @@ forall (cur_num_pre: Z) (num_pre: Z) (r2_pre: Z) (r1_pre: Z) (c2: Constraint) (c
   &&  [| (0 <= cur_num_pre) |] 
   &&  [| (cur_num_pre < (num_pre + 1 )) |] 
   &&  [| ((num_pre + 1 ) <= INT_MAX) |] 
+  &&  [| (r1_pre <> 0) |] 
+  &&  [| (r2_pre <> 0) |] 
   &&  [| ((coef_Znth (cur_num_pre) (c1) (0)) > 0) |] 
   &&  [| ((coef_Znth (cur_num_pre) (c1) (0)) <= INT_MAX) |] 
   &&  [| ((coef_Znth (cur_num_pre) (c2) (0)) < 0) |] 
@@ -3675,6 +3755,8 @@ forall (cur_num_pre: Z) (num_pre: Z) (r2_pre: Z) (r1_pre: Z) (c2: Constraint) (c
   &&  [| (0 <= cur_num_pre) |] 
   &&  [| (cur_num_pre < (num_pre + 1 )) |] 
   &&  [| ((num_pre + 1 ) <= INT_MAX) |] 
+  &&  [| (r1_pre <> 0) |] 
+  &&  [| (r2_pre <> 0) |] 
   &&  [| ((coef_Znth (cur_num_pre) (c1) (0)) > 0) |] 
   &&  [| ((coef_Znth (cur_num_pre) (c1) (0)) <= INT_MAX) |] 
   &&  [| ((coef_Znth (cur_num_pre) (c2) (0)) < 0) |] 
@@ -3717,6 +3799,8 @@ forall (cur_num_pre: Z) (num_pre: Z) (r2_pre: Z) (r1_pre: Z) (c2: Constraint) (c
   &&  [| (0 <= cur_num_pre) |] 
   &&  [| (cur_num_pre < (num_pre + 1 )) |] 
   &&  [| ((num_pre + 1 ) <= INT_MAX) |] 
+  &&  [| (r1_pre <> 0) |] 
+  &&  [| (r2_pre <> 0) |] 
   &&  [| ((coef_Znth (cur_num_pre) (c1) (0)) > 0) |] 
   &&  [| ((coef_Znth (cur_num_pre) (c1) (0)) <= INT_MAX) |] 
   &&  [| ((coef_Znth (cur_num_pre) (c2) (0)) < 0) |] 
@@ -3756,6 +3840,8 @@ forall (cur_num_pre: Z) (num_pre: Z) (r2_pre: Z) (r1_pre: Z) (c2: Constraint) (c
   &&  [| (0 <= cur_num_pre) |] 
   &&  [| (cur_num_pre < (num_pre + 1 )) |] 
   &&  [| ((num_pre + 1 ) <= INT_MAX) |] 
+  &&  [| (r1_pre <> 0) |] 
+  &&  [| (r2_pre <> 0) |] 
   &&  [| ((coef_Znth (cur_num_pre) (c1) (0)) > 0) |] 
   &&  [| ((coef_Znth (cur_num_pre) (c1) (0)) <= INT_MAX) |] 
   &&  [| ((coef_Znth (cur_num_pre) (c2) (0)) < 0) |] 
@@ -3805,7 +3891,7 @@ forall (init_pre: Z) (cur_num_pre: Z) (num_pre: Z) (r2_pre: Z) (r1_pre: Z) (l_in
 .
 
 Definition generate_new_constraint_list_safety_wit_2 := 
-forall (init_pre: Z) (cur_num_pre: Z) (num_pre: Z) (r2_pre: Z) (r1_pre: Z) (l_init: (@list Constraint)) (l2: (@list Constraint)) (l1: (@list Constraint)) (n: Z) (p1_2: Z) (l3_2: (@list Constraint)) (l4_2: (@list Constraint)) (l11_2: (@list Constraint)) (l12_2: (@list Constraint)) (x: Constraint) (l13: (@list Constraint)) (res: Z) (p2: Z) (p1_next: Z) (p1_coef: Z) (l3: (@list Constraint)) (l4: (@list Constraint)) (p1: Z) (l21: (@list Constraint)) (l22: (@list Constraint)) (l11: (@list Constraint)) (x1: Constraint) (l12: (@list Constraint)) ,
+forall (init_pre: Z) (cur_num_pre: Z) (num_pre: Z) (r2_pre: Z) (r1_pre: Z) (l_init: (@list Constraint)) (l2: (@list Constraint)) (l1: (@list Constraint)) (n: Z) (p1_2: Z) (l3_2: (@list Constraint)) (l4_2: (@list Constraint)) (l11_2: (@list Constraint)) (l12_2: (@list Constraint)) (p1_coef_2: Z) (x: Constraint) (l13: (@list Constraint)) (res: Z) (p2: Z) (p1_next: Z) (p1_coef: Z) (l3: (@list Constraint)) (l4: (@list Constraint)) (p1: Z) (l21: (@list Constraint)) (l22: (@list Constraint)) (l11: (@list Constraint)) (x1: Constraint) (l12: (@list Constraint)) ,
   [| (n = (num_pre + 1 )) |] 
   &&  [| (0 <= cur_num_pre) |] 
   &&  [| (cur_num_pre < n) |] 
@@ -3817,7 +3903,9 @@ forall (init_pre: Z) (cur_num_pre: Z) (num_pre: Z) (r2_pre: Z) (r1_pre: Z) (l_in
   &&  [| (generate_new_constraints_partial (Zto_nat ((cur_num_pre - 1 ))) l11 x1 l21 l22 l4 ) |] 
   &&  [| (l3 = (app (l4) (l_init))) |] 
   &&  [| (LP_abs_in_int_range n l3 ) |] 
+  &&  [| (p1_coef <> 0) |] 
   &&  [| (l12_2 = (cons (x) (l13))) |] 
+  &&  [| (p1_coef_2 <> 0) |] 
   &&  [| (p1_2 <> 0) |] 
   &&  [| (n = (num_pre + 1 )) |] 
   &&  [| (0 <= cur_num_pre) |] 
@@ -3843,8 +3931,8 @@ forall (init_pre: Z) (cur_num_pre: Z) (num_pre: Z) (r2_pre: Z) (r1_pre: Z) (l_in
   **  ((( &( "r1" ) )) # Ptr  |-> r1_pre)
   **  ((( &( "r2" ) )) # Ptr  |-> r2_pre)
   **  ((( &( "init" ) )) # Ptr  |-> init_pre)
-  **  (InequList_seg r1_pre p1 n l11 )
   **  ((&((p1)  # "InequList" ->ₛ "coef")) # Ptr  |-> p1_coef)
+  **  (InequList_seg r1_pre p1 n l11 )
   **  (coef_array p1_coef n x1 )
   **  ((&((p1)  # "InequList" ->ₛ "next")) # Ptr  |-> p1_next)
   **  (InequList p1_next n l12 )
@@ -3859,9 +3947,10 @@ forall (init_pre: Z) (cur_num_pre: Z) (num_pre: Z) (r2_pre: Z) (r1_pre: Z) (l_in
 .
 
 Definition generate_new_constraint_list_safety_wit_3 := 
-forall (init_pre: Z) (cur_num_pre: Z) (num_pre: Z) (r2_pre: Z) (r1_pre: Z) (l_init: (@list Constraint)) (l2: (@list Constraint)) (l1: (@list Constraint)) (n: Z) (p1: Z) (l3: (@list Constraint)) (l4: (@list Constraint)) (l11: (@list Constraint)) (l12: (@list Constraint)) (x: Constraint) (l13: (@list Constraint)) (res: Z) (p2: Z) (p1_next: Z) (p1_coef: Z) (l3_2: (@list Constraint)) (l4_2: (@list Constraint)) (p1_2: Z) (l21: (@list Constraint)) (l22: (@list Constraint)) (l11_2: (@list Constraint)) (x1: Constraint) (l12_2: (@list Constraint)) (p2_next: Z) (p2_coef: Z) (x_2: Constraint) (l23: (@list Constraint)) (retval: Z) ,
+forall (init_pre: Z) (cur_num_pre: Z) (num_pre: Z) (r2_pre: Z) (r1_pre: Z) (l_init: (@list Constraint)) (l2: (@list Constraint)) (l1: (@list Constraint)) (n: Z) (p1: Z) (l3: (@list Constraint)) (l4: (@list Constraint)) (l11: (@list Constraint)) (l12: (@list Constraint)) (p1_coef: Z) (x: Constraint) (l13: (@list Constraint)) (res: Z) (p2: Z) (p1_next: Z) (p1_coef_2: Z) (l3_2: (@list Constraint)) (l4_2: (@list Constraint)) (p1_2: Z) (l21: (@list Constraint)) (l22: (@list Constraint)) (l11_2: (@list Constraint)) (x1: Constraint) (l12_2: (@list Constraint)) (p2_next: Z) (p2_coef: Z) (x_2: Constraint) (l23: (@list Constraint)) (retval: Z) ,
   [| (retval = 0) |] 
   &&  [| (l22 = (cons (x_2) (l23))) |] 
+  &&  [| (p2_coef <> 0) |] 
   &&  [| (p2 <> 0) |] 
   &&  [| (n = (num_pre + 1 )) |] 
   &&  [| (0 <= cur_num_pre) |] 
@@ -3874,7 +3963,9 @@ forall (init_pre: Z) (cur_num_pre: Z) (num_pre: Z) (r2_pre: Z) (r1_pre: Z) (l_in
   &&  [| (generate_new_constraints_partial (Zto_nat ((cur_num_pre - 1 ))) l11_2 x1 l21 l22 l4_2 ) |] 
   &&  [| (l3_2 = (app (l4_2) (l_init))) |] 
   &&  [| (LP_abs_in_int_range n l3_2 ) |] 
+  &&  [| (p1_coef_2 <> 0) |] 
   &&  [| (l12 = (cons (x) (l13))) |] 
+  &&  [| (p1_coef <> 0) |] 
   &&  [| (p1 <> 0) |] 
   &&  [| (n = (num_pre + 1 )) |] 
   &&  [| (0 <= cur_num_pre) |] 
@@ -3894,13 +3985,13 @@ forall (init_pre: Z) (cur_num_pre: Z) (num_pre: Z) (r2_pre: Z) (r1_pre: Z) (l_in
   &&  [| (LP_abs_in_int_range n l1 ) |] 
   &&  [| (LP_abs_in_int_range n l2 ) |] 
   &&  [| (LP_abs_in_int_range n l_init ) |]
-  &&  (coef_array p1_coef (num_pre + 1 ) x1 )
+  &&  (coef_array p1_coef_2 (num_pre + 1 ) x1 )
   **  (coef_array p2_coef (num_pre + 1 ) x_2 )
   **  ((( &( "tmp" ) )) # Ptr  |-> retval)
   **  ((( &( "p2" ) )) # Ptr  |-> p2)
+  **  ((&((p2)  # "InequList" ->ₛ "coef")) # Ptr  |-> p2_coef)
   **  ((( &( "r2" ) )) # Ptr  |-> r2_pre)
   **  (InequList_seg r2_pre p2 n l21 )
-  **  ((&((p2)  # "InequList" ->ₛ "coef")) # Ptr  |-> p2_coef)
   **  ((&((p2)  # "InequList" ->ₛ "next")) # Ptr  |-> p2_next)
   **  (InequList p2_next n l23 )
   **  ((( &( "num" ) )) # Int  |-> num_pre)
@@ -3908,8 +3999,8 @@ forall (init_pre: Z) (cur_num_pre: Z) (num_pre: Z) (r2_pre: Z) (r1_pre: Z) (l_in
   **  ((( &( "p1" ) )) # Ptr  |-> p1_2)
   **  ((( &( "r1" ) )) # Ptr  |-> r1_pre)
   **  ((( &( "init" ) )) # Ptr  |-> init_pre)
+  **  ((&((p1_2)  # "InequList" ->ₛ "coef")) # Ptr  |-> p1_coef_2)
   **  (InequList_seg r1_pre p1_2 n l11_2 )
-  **  ((&((p1_2)  # "InequList" ->ₛ "coef")) # Ptr  |-> p1_coef)
   **  ((&((p1_2)  # "InequList" ->ₛ "next")) # Ptr  |-> p1_next)
   **  (InequList p1_next n l12_2 )
   **  ((( &( "res" ) )) # Ptr  |-> res)
@@ -3920,10 +4011,11 @@ forall (init_pre: Z) (cur_num_pre: Z) (num_pre: Z) (r2_pre: Z) (r1_pre: Z) (l_in
 .
 
 Definition generate_new_constraint_list_safety_wit_4 := 
-forall (init_pre: Z) (cur_num_pre: Z) (num_pre: Z) (r2_pre: Z) (r1_pre: Z) (l_init: (@list Constraint)) (l2: (@list Constraint)) (l1: (@list Constraint)) (n: Z) (p1: Z) (l3: (@list Constraint)) (l4: (@list Constraint)) (l11: (@list Constraint)) (l12: (@list Constraint)) (x: Constraint) (l13: (@list Constraint)) (res: Z) (p2: Z) (p1_next: Z) (p1_coef: Z) (l3_2: (@list Constraint)) (l4_2: (@list Constraint)) (p1_2: Z) (l21: (@list Constraint)) (l22: (@list Constraint)) (l11_2: (@list Constraint)) (x1: Constraint) (l12_2: (@list Constraint)) (p2_next: Z) (p2_coef: Z) (x_2: Constraint) (l23: (@list Constraint)) (retval: Z) ,
+forall (init_pre: Z) (cur_num_pre: Z) (num_pre: Z) (r2_pre: Z) (r1_pre: Z) (l_init: (@list Constraint)) (l2: (@list Constraint)) (l1: (@list Constraint)) (n: Z) (p1: Z) (l3: (@list Constraint)) (l4: (@list Constraint)) (l11: (@list Constraint)) (l12: (@list Constraint)) (p1_coef: Z) (x: Constraint) (l13: (@list Constraint)) (res: Z) (p2: Z) (p1_next: Z) (p1_coef_2: Z) (l3_2: (@list Constraint)) (l4_2: (@list Constraint)) (p1_2: Z) (l21: (@list Constraint)) (l22: (@list Constraint)) (l11_2: (@list Constraint)) (x1: Constraint) (l12_2: (@list Constraint)) (p2_next: Z) (p2_coef: Z) (x_2: Constraint) (l23: (@list Constraint)) (retval: Z) ,
   [| (retval <> 0) |] 
   &&  [| (retval = 0) |] 
   &&  [| (l22 = (cons (x_2) (l23))) |] 
+  &&  [| (p2_coef <> 0) |] 
   &&  [| (p2 <> 0) |] 
   &&  [| (n = (num_pre + 1 )) |] 
   &&  [| (0 <= cur_num_pre) |] 
@@ -3936,7 +4028,9 @@ forall (init_pre: Z) (cur_num_pre: Z) (num_pre: Z) (r2_pre: Z) (r1_pre: Z) (l_in
   &&  [| (generate_new_constraints_partial (Zto_nat ((cur_num_pre - 1 ))) l11_2 x1 l21 l22 l4_2 ) |] 
   &&  [| (l3_2 = (app (l4_2) (l_init))) |] 
   &&  [| (LP_abs_in_int_range n l3_2 ) |] 
+  &&  [| (p1_coef_2 <> 0) |] 
   &&  [| (l12 = (cons (x) (l13))) |] 
+  &&  [| (p1_coef <> 0) |] 
   &&  [| (p1 <> 0) |] 
   &&  [| (n = (num_pre + 1 )) |] 
   &&  [| (0 <= cur_num_pre) |] 
@@ -3956,13 +4050,13 @@ forall (init_pre: Z) (cur_num_pre: Z) (num_pre: Z) (r2_pre: Z) (r1_pre: Z) (l_in
   &&  [| (LP_abs_in_int_range n l1 ) |] 
   &&  [| (LP_abs_in_int_range n l2 ) |] 
   &&  [| (LP_abs_in_int_range n l_init ) |]
-  &&  (coef_array p1_coef (num_pre + 1 ) x1 )
+  &&  (coef_array p1_coef_2 (num_pre + 1 ) x1 )
   **  (coef_array p2_coef (num_pre + 1 ) x_2 )
   **  ((( &( "tmp" ) )) # Ptr  |-> retval)
   **  ((( &( "p2" ) )) # Ptr  |-> p2)
+  **  ((&((p2)  # "InequList" ->ₛ "coef")) # Ptr  |-> p2_coef)
   **  ((( &( "r2" ) )) # Ptr  |-> r2_pre)
   **  (InequList_seg r2_pre p2 n l21 )
-  **  ((&((p2)  # "InequList" ->ₛ "coef")) # Ptr  |-> p2_coef)
   **  ((&((p2)  # "InequList" ->ₛ "next")) # Ptr  |-> p2_next)
   **  (InequList p2_next n l23 )
   **  ((( &( "num" ) )) # Int  |-> num_pre)
@@ -3970,8 +4064,8 @@ forall (init_pre: Z) (cur_num_pre: Z) (num_pre: Z) (r2_pre: Z) (r1_pre: Z) (l_in
   **  ((( &( "p1" ) )) # Ptr  |-> p1_2)
   **  ((( &( "r1" ) )) # Ptr  |-> r1_pre)
   **  ((( &( "init" ) )) # Ptr  |-> init_pre)
+  **  ((&((p1_2)  # "InequList" ->ₛ "coef")) # Ptr  |-> p1_coef_2)
   **  (InequList_seg r1_pre p1_2 n l11_2 )
-  **  ((&((p1_2)  # "InequList" ->ₛ "coef")) # Ptr  |-> p1_coef)
   **  ((&((p1_2)  # "InequList" ->ₛ "next")) # Ptr  |-> p1_next)
   **  (InequList p1_next n l12_2 )
   **  ((( &( "res" ) )) # Ptr  |-> res)
@@ -3981,11 +4075,12 @@ forall (init_pre: Z) (cur_num_pre: Z) (num_pre: Z) (r2_pre: Z) (r1_pre: Z) (l_in
 .
 
 Definition generate_new_constraint_list_safety_wit_5 := 
-forall (init_pre: Z) (cur_num_pre: Z) (num_pre: Z) (r2_pre: Z) (r1_pre: Z) (l_init: (@list Constraint)) (l2: (@list Constraint)) (l1: (@list Constraint)) (n: Z) (p1: Z) (l3: (@list Constraint)) (l4: (@list Constraint)) (l11: (@list Constraint)) (l12: (@list Constraint)) (x: Constraint) (l13: (@list Constraint)) (res: Z) (p2: Z) (p1_next: Z) (p1_coef: Z) (l3_2: (@list Constraint)) (l4_2: (@list Constraint)) (p1_2: Z) (l21: (@list Constraint)) (l22: (@list Constraint)) (l11_2: (@list Constraint)) (x1: Constraint) (l12_2: (@list Constraint)) (p2_next: Z) (p2_coef: Z) (x_2: Constraint) (l23: (@list Constraint)) (c3: Constraint) (retval: Z) ,
+forall (init_pre: Z) (cur_num_pre: Z) (num_pre: Z) (r2_pre: Z) (r1_pre: Z) (l_init: (@list Constraint)) (l2: (@list Constraint)) (l1: (@list Constraint)) (n: Z) (p1: Z) (l3: (@list Constraint)) (l4: (@list Constraint)) (l11: (@list Constraint)) (l12: (@list Constraint)) (p1_coef: Z) (x: Constraint) (l13: (@list Constraint)) (res: Z) (p2: Z) (p1_next: Z) (p1_coef_2: Z) (l3_2: (@list Constraint)) (l4_2: (@list Constraint)) (p1_2: Z) (l21: (@list Constraint)) (l22: (@list Constraint)) (l11_2: (@list Constraint)) (x1: Constraint) (l12_2: (@list Constraint)) (p2_next: Z) (p2_coef: Z) (x_2: Constraint) (l23: (@list Constraint)) (c3: Constraint) (retval: Z) ,
   [| (retval <> 0) |] 
   &&  [| (generate_new_constraint (Zto_nat ((cur_num_pre - 1 ))) x1 x_2 c3 ) |] 
   &&  [| (abs_in_int_range (num_pre + 1 ) c3 ) |] 
   &&  [| (l22 = (cons (x_2) (l23))) |] 
+  &&  [| (p2_coef <> 0) |] 
   &&  [| (p2 <> 0) |] 
   &&  [| (n = (num_pre + 1 )) |] 
   &&  [| (0 <= cur_num_pre) |] 
@@ -3998,7 +4093,9 @@ forall (init_pre: Z) (cur_num_pre: Z) (num_pre: Z) (r2_pre: Z) (r1_pre: Z) (l_in
   &&  [| (generate_new_constraints_partial (Zto_nat ((cur_num_pre - 1 ))) l11_2 x1 l21 l22 l4_2 ) |] 
   &&  [| (l3_2 = (app (l4_2) (l_init))) |] 
   &&  [| (LP_abs_in_int_range n l3_2 ) |] 
+  &&  [| (p1_coef_2 <> 0) |] 
   &&  [| (l12 = (cons (x) (l13))) |] 
+  &&  [| (p1_coef <> 0) |] 
   &&  [| (p1 <> 0) |] 
   &&  [| (n = (num_pre + 1 )) |] 
   &&  [| (0 <= cur_num_pre) |] 
@@ -4018,14 +4115,14 @@ forall (init_pre: Z) (cur_num_pre: Z) (num_pre: Z) (r2_pre: Z) (r1_pre: Z) (l_in
   &&  [| (LP_abs_in_int_range n l1 ) |] 
   &&  [| (LP_abs_in_int_range n l2 ) |] 
   &&  [| (LP_abs_in_int_range n l_init ) |]
-  &&  (coef_array p1_coef (num_pre + 1 ) x1 )
+  &&  (coef_array p1_coef_2 (num_pre + 1 ) x1 )
   **  (coef_array p2_coef (num_pre + 1 ) x_2 )
   **  (coef_array retval (num_pre + 1 ) c3 )
   **  ((( &( "tmp" ) )) # Ptr  |-> retval)
   **  ((( &( "p2" ) )) # Ptr  |-> p2)
+  **  ((&((p2)  # "InequList" ->ₛ "coef")) # Ptr  |-> p2_coef)
   **  ((( &( "r2" ) )) # Ptr  |-> r2_pre)
   **  (InequList_seg r2_pre p2 n l21 )
-  **  ((&((p2)  # "InequList" ->ₛ "coef")) # Ptr  |-> p2_coef)
   **  ((&((p2)  # "InequList" ->ₛ "next")) # Ptr  |-> p2_next)
   **  (InequList p2_next n l23 )
   **  ((( &( "num" ) )) # Int  |-> num_pre)
@@ -4033,8 +4130,8 @@ forall (init_pre: Z) (cur_num_pre: Z) (num_pre: Z) (r2_pre: Z) (r1_pre: Z) (l_in
   **  ((( &( "p1" ) )) # Ptr  |-> p1_2)
   **  ((( &( "r1" ) )) # Ptr  |-> r1_pre)
   **  ((( &( "init" ) )) # Ptr  |-> init_pre)
+  **  ((&((p1_2)  # "InequList" ->ₛ "coef")) # Ptr  |-> p1_coef_2)
   **  (InequList_seg r1_pre p1_2 n l11_2 )
-  **  ((&((p1_2)  # "InequList" ->ₛ "coef")) # Ptr  |-> p1_coef)
   **  ((&((p1_2)  # "InequList" ->ₛ "next")) # Ptr  |-> p1_next)
   **  (InequList p1_next n l12_2 )
   **  ((( &( "res" ) )) # Ptr  |-> res)
@@ -4045,12 +4142,13 @@ forall (init_pre: Z) (cur_num_pre: Z) (num_pre: Z) (r2_pre: Z) (r1_pre: Z) (l_in
 .
 
 Definition generate_new_constraint_list_safety_wit_6 := 
-forall (init_pre: Z) (cur_num_pre: Z) (num_pre: Z) (r2_pre: Z) (r1_pre: Z) (l_init: (@list Constraint)) (l2: (@list Constraint)) (l1: (@list Constraint)) (n: Z) (p1: Z) (l3: (@list Constraint)) (l4: (@list Constraint)) (l11: (@list Constraint)) (l12: (@list Constraint)) (x: Constraint) (l13: (@list Constraint)) (res: Z) (p2: Z) (p1_next: Z) (p1_coef: Z) (l3_2: (@list Constraint)) (l4_2: (@list Constraint)) (p1_2: Z) (l21: (@list Constraint)) (l22: (@list Constraint)) (l11_2: (@list Constraint)) (x1: Constraint) (l12_2: (@list Constraint)) (p2_next: Z) (p2_coef: Z) (x_2: Constraint) (l23: (@list Constraint)) (c3: Constraint) (retval: Z) ,
+forall (init_pre: Z) (cur_num_pre: Z) (num_pre: Z) (r2_pre: Z) (r1_pre: Z) (l_init: (@list Constraint)) (l2: (@list Constraint)) (l1: (@list Constraint)) (n: Z) (p1: Z) (l3: (@list Constraint)) (l4: (@list Constraint)) (l11: (@list Constraint)) (l12: (@list Constraint)) (p1_coef: Z) (x: Constraint) (l13: (@list Constraint)) (res: Z) (p2: Z) (p1_next: Z) (p1_coef_2: Z) (l3_2: (@list Constraint)) (l4_2: (@list Constraint)) (p1_2: Z) (l21: (@list Constraint)) (l22: (@list Constraint)) (l11_2: (@list Constraint)) (x1: Constraint) (l12_2: (@list Constraint)) (p2_next: Z) (p2_coef: Z) (x_2: Constraint) (l23: (@list Constraint)) (c3: Constraint) (retval: Z) ,
   [| (retval = 0) |] 
   &&  [| (retval <> 0) |] 
   &&  [| (generate_new_constraint (Zto_nat ((cur_num_pre - 1 ))) x1 x_2 c3 ) |] 
   &&  [| (abs_in_int_range (num_pre + 1 ) c3 ) |] 
   &&  [| (l22 = (cons (x_2) (l23))) |] 
+  &&  [| (p2_coef <> 0) |] 
   &&  [| (p2 <> 0) |] 
   &&  [| (n = (num_pre + 1 )) |] 
   &&  [| (0 <= cur_num_pre) |] 
@@ -4063,7 +4161,9 @@ forall (init_pre: Z) (cur_num_pre: Z) (num_pre: Z) (r2_pre: Z) (r1_pre: Z) (l_in
   &&  [| (generate_new_constraints_partial (Zto_nat ((cur_num_pre - 1 ))) l11_2 x1 l21 l22 l4_2 ) |] 
   &&  [| (l3_2 = (app (l4_2) (l_init))) |] 
   &&  [| (LP_abs_in_int_range n l3_2 ) |] 
+  &&  [| (p1_coef_2 <> 0) |] 
   &&  [| (l12 = (cons (x) (l13))) |] 
+  &&  [| (p1_coef <> 0) |] 
   &&  [| (p1 <> 0) |] 
   &&  [| (n = (num_pre + 1 )) |] 
   &&  [| (0 <= cur_num_pre) |] 
@@ -4083,14 +4183,14 @@ forall (init_pre: Z) (cur_num_pre: Z) (num_pre: Z) (r2_pre: Z) (r1_pre: Z) (l_in
   &&  [| (LP_abs_in_int_range n l1 ) |] 
   &&  [| (LP_abs_in_int_range n l2 ) |] 
   &&  [| (LP_abs_in_int_range n l_init ) |]
-  &&  (coef_array p1_coef (num_pre + 1 ) x1 )
+  &&  (coef_array p1_coef_2 (num_pre + 1 ) x1 )
   **  (coef_array p2_coef (num_pre + 1 ) x_2 )
   **  (coef_array retval (num_pre + 1 ) c3 )
   **  ((( &( "tmp" ) )) # Ptr  |-> retval)
   **  ((( &( "p2" ) )) # Ptr  |-> p2)
+  **  ((&((p2)  # "InequList" ->ₛ "coef")) # Ptr  |-> p2_coef)
   **  ((( &( "r2" ) )) # Ptr  |-> r2_pre)
   **  (InequList_seg r2_pre p2 n l21 )
-  **  ((&((p2)  # "InequList" ->ₛ "coef")) # Ptr  |-> p2_coef)
   **  ((&((p2)  # "InequList" ->ₛ "next")) # Ptr  |-> p2_next)
   **  (InequList p2_next n l23 )
   **  ((( &( "num" ) )) # Int  |-> num_pre)
@@ -4098,8 +4198,8 @@ forall (init_pre: Z) (cur_num_pre: Z) (num_pre: Z) (r2_pre: Z) (r1_pre: Z) (l_in
   **  ((( &( "p1" ) )) # Ptr  |-> p1_2)
   **  ((( &( "r1" ) )) # Ptr  |-> r1_pre)
   **  ((( &( "init" ) )) # Ptr  |-> init_pre)
+  **  ((&((p1_2)  # "InequList" ->ₛ "coef")) # Ptr  |-> p1_coef_2)
   **  (InequList_seg r1_pre p1_2 n l11_2 )
-  **  ((&((p1_2)  # "InequList" ->ₛ "coef")) # Ptr  |-> p1_coef)
   **  ((&((p1_2)  # "InequList" ->ₛ "next")) # Ptr  |-> p1_next)
   **  (InequList p1_next n l12_2 )
   **  ((( &( "res" ) )) # Ptr  |-> res)
@@ -4109,10 +4209,11 @@ forall (init_pre: Z) (cur_num_pre: Z) (num_pre: Z) (r2_pre: Z) (r1_pre: Z) (l_in
 .
 
 Definition generate_new_constraint_list_safety_wit_7 := 
-forall (init_pre: Z) (cur_num_pre: Z) (num_pre: Z) (r2_pre: Z) (r1_pre: Z) (l_init: (@list Constraint)) (l2: (@list Constraint)) (l1: (@list Constraint)) (n: Z) (p1: Z) (l3: (@list Constraint)) (l4: (@list Constraint)) (l11: (@list Constraint)) (l12: (@list Constraint)) (x: Constraint) (l13: (@list Constraint)) (res: Z) (p2: Z) (p1_next: Z) (p1_coef: Z) (l3_2: (@list Constraint)) (l4_2: (@list Constraint)) (p1_2: Z) (l21: (@list Constraint)) (l22: (@list Constraint)) (l11_2: (@list Constraint)) (x1: Constraint) (l12_2: (@list Constraint)) (p2_next: Z) (p2_coef: Z) (x_2: Constraint) (l23: (@list Constraint)) (retval: Z) ,
+forall (init_pre: Z) (cur_num_pre: Z) (num_pre: Z) (r2_pre: Z) (r1_pre: Z) (l_init: (@list Constraint)) (l2: (@list Constraint)) (l1: (@list Constraint)) (n: Z) (p1: Z) (l3: (@list Constraint)) (l4: (@list Constraint)) (l11: (@list Constraint)) (l12: (@list Constraint)) (p1_coef: Z) (x: Constraint) (l13: (@list Constraint)) (res: Z) (p2: Z) (p1_next: Z) (p1_coef_2: Z) (l3_2: (@list Constraint)) (l4_2: (@list Constraint)) (p1_2: Z) (l21: (@list Constraint)) (l22: (@list Constraint)) (l11_2: (@list Constraint)) (x1: Constraint) (l12_2: (@list Constraint)) (p2_next: Z) (p2_coef: Z) (x_2: Constraint) (l23: (@list Constraint)) (retval: Z) ,
   [| (retval = 0) |] 
   &&  [| (retval = 0) |] 
   &&  [| (l22 = (cons (x_2) (l23))) |] 
+  &&  [| (p2_coef <> 0) |] 
   &&  [| (p2 <> 0) |] 
   &&  [| (n = (num_pre + 1 )) |] 
   &&  [| (0 <= cur_num_pre) |] 
@@ -4125,7 +4226,9 @@ forall (init_pre: Z) (cur_num_pre: Z) (num_pre: Z) (r2_pre: Z) (r1_pre: Z) (l_in
   &&  [| (generate_new_constraints_partial (Zto_nat ((cur_num_pre - 1 ))) l11_2 x1 l21 l22 l4_2 ) |] 
   &&  [| (l3_2 = (app (l4_2) (l_init))) |] 
   &&  [| (LP_abs_in_int_range n l3_2 ) |] 
+  &&  [| (p1_coef_2 <> 0) |] 
   &&  [| (l12 = (cons (x) (l13))) |] 
+  &&  [| (p1_coef <> 0) |] 
   &&  [| (p1 <> 0) |] 
   &&  [| (n = (num_pre + 1 )) |] 
   &&  [| (0 <= cur_num_pre) |] 
@@ -4145,13 +4248,13 @@ forall (init_pre: Z) (cur_num_pre: Z) (num_pre: Z) (r2_pre: Z) (r1_pre: Z) (l_in
   &&  [| (LP_abs_in_int_range n l1 ) |] 
   &&  [| (LP_abs_in_int_range n l2 ) |] 
   &&  [| (LP_abs_in_int_range n l_init ) |]
-  &&  (coef_array p1_coef (num_pre + 1 ) x1 )
+  &&  (coef_array p1_coef_2 (num_pre + 1 ) x1 )
   **  (coef_array p2_coef (num_pre + 1 ) x_2 )
   **  ((( &( "tmp" ) )) # Ptr  |-> retval)
   **  ((( &( "p2" ) )) # Ptr  |-> p2)
+  **  ((&((p2)  # "InequList" ->ₛ "coef")) # Ptr  |-> p2_coef)
   **  ((( &( "r2" ) )) # Ptr  |-> r2_pre)
   **  (InequList_seg r2_pre p2 n l21 )
-  **  ((&((p2)  # "InequList" ->ₛ "coef")) # Ptr  |-> p2_coef)
   **  ((&((p2)  # "InequList" ->ₛ "next")) # Ptr  |-> p2_next)
   **  (InequList p2_next n l23 )
   **  ((( &( "num" ) )) # Int  |-> num_pre)
@@ -4159,8 +4262,8 @@ forall (init_pre: Z) (cur_num_pre: Z) (num_pre: Z) (r2_pre: Z) (r1_pre: Z) (l_in
   **  ((( &( "p1" ) )) # Ptr  |-> p1_2)
   **  ((( &( "r1" ) )) # Ptr  |-> r1_pre)
   **  ((( &( "init" ) )) # Ptr  |-> init_pre)
+  **  ((&((p1_2)  # "InequList" ->ₛ "coef")) # Ptr  |-> p1_coef_2)
   **  (InequList_seg r1_pre p1_2 n l11_2 )
-  **  ((&((p1_2)  # "InequList" ->ₛ "coef")) # Ptr  |-> p1_coef)
   **  ((&((p1_2)  # "InequList" ->ₛ "next")) # Ptr  |-> p1_next)
   **  (InequList p1_next n l12_2 )
   **  ((( &( "res" ) )) # Ptr  |-> res)
@@ -4212,6 +4315,7 @@ forall (init_pre: Z) (cur_num_pre: Z) (num_pre: Z) (r2_pre: Z) (r1_pre: Z) (l_in
 Definition generate_new_constraint_list_entail_wit_2 := 
 forall (cur_num_pre: Z) (num_pre: Z) (r2_pre: Z) (r1_pre: Z) (l_init: (@list Constraint)) (l2: (@list Constraint)) (l1: (@list Constraint)) (n: Z) (res: Z) (p1: Z) (l3_2: (@list Constraint)) (l4_2: (@list Constraint)) (l11_2: (@list Constraint)) (l12_2: (@list Constraint)) (p1_next_2: Z) (p1_coef_2: Z) (x: Constraint) (l13: (@list Constraint)) ,
   [| (l12_2 = (cons (x) (l13))) |] 
+  &&  [| (p1_coef_2 <> 0) |] 
   &&  [| (p1 <> 0) |] 
   &&  [| (n = (num_pre + 1 )) |] 
   &&  [| (0 <= cur_num_pre) |] 
@@ -4231,8 +4335,8 @@ forall (cur_num_pre: Z) (num_pre: Z) (r2_pre: Z) (r1_pre: Z) (l_init: (@list Con
   &&  [| (LP_abs_in_int_range n l1 ) |] 
   &&  [| (LP_abs_in_int_range n l2 ) |] 
   &&  [| (LP_abs_in_int_range n l_init ) |]
-  &&  (InequList_seg r1_pre p1 n l11_2 )
-  **  ((&((p1)  # "InequList" ->ₛ "coef")) # Ptr  |-> p1_coef_2)
+  &&  ((&((p1)  # "InequList" ->ₛ "coef")) # Ptr  |-> p1_coef_2)
+  **  (InequList_seg r1_pre p1 n l11_2 )
   **  (coef_array p1_coef_2 n x )
   **  ((&((p1)  # "InequList" ->ₛ "next")) # Ptr  |-> p1_next_2)
   **  (InequList p1_next_2 n l13 )
@@ -4251,7 +4355,9 @@ forall (cur_num_pre: Z) (num_pre: Z) (r2_pre: Z) (r1_pre: Z) (l_init: (@list Con
   &&  [| (generate_new_constraints_partial (Zto_nat ((cur_num_pre - 1 ))) l11 x1 l21 l22 l4 ) |] 
   &&  [| (l3 = (app (l4) (l_init))) |] 
   &&  [| (LP_abs_in_int_range n l3 ) |] 
+  &&  [| (p1_coef <> 0) |] 
   &&  [| (l12_2 = (cons (x) (l13))) |] 
+  &&  [| (p1_coef_2 <> 0) |] 
   &&  [| (p1 <> 0) |] 
   &&  [| (n = (num_pre + 1 )) |] 
   &&  [| (0 <= cur_num_pre) |] 
@@ -4271,8 +4377,8 @@ forall (cur_num_pre: Z) (num_pre: Z) (r2_pre: Z) (r1_pre: Z) (l_init: (@list Con
   &&  [| (LP_abs_in_int_range n l1 ) |] 
   &&  [| (LP_abs_in_int_range n l2 ) |] 
   &&  [| (LP_abs_in_int_range n l_init ) |]
-  &&  (InequList_seg r1_pre p1 n l11 )
-  **  ((&((p1)  # "InequList" ->ₛ "coef")) # Ptr  |-> p1_coef)
+  &&  ((&((p1)  # "InequList" ->ₛ "coef")) # Ptr  |-> p1_coef)
+  **  (InequList_seg r1_pre p1 n l11 )
   **  (coef_array p1_coef n x1 )
   **  ((&((p1)  # "InequList" ->ₛ "next")) # Ptr  |-> p1_next)
   **  (InequList p1_next n l12 )
@@ -4282,12 +4388,13 @@ forall (cur_num_pre: Z) (num_pre: Z) (r2_pre: Z) (r1_pre: Z) (l_init: (@list Con
 .
 
 Definition generate_new_constraint_list_entail_wit_3 := 
-forall (cur_num_pre: Z) (num_pre: Z) (r2_pre: Z) (r1_pre: Z) (l_init: (@list Constraint)) (l2: (@list Constraint)) (l1: (@list Constraint)) (n: Z) (p1: Z) (l3_2: (@list Constraint)) (l4_2: (@list Constraint)) (l11_2: (@list Constraint)) (l12_2: (@list Constraint)) (x: Constraint) (l13: (@list Constraint)) (p2: Z) (p1_next_2: Z) (p1_coef_2: Z) (l3_3: (@list Constraint)) (l4_3: (@list Constraint)) (p1_2: Z) (l21_2: (@list Constraint)) (l22_2: (@list Constraint)) (l11_3: (@list Constraint)) (x1_2: Constraint) (l12_3: (@list Constraint)) (p2_next: Z) (p2_coef: Z) (x_2: Constraint) (l23: (@list Constraint)) (c3: Constraint) (retval_2: Z) (retval: Z) ,
+forall (cur_num_pre: Z) (num_pre: Z) (r2_pre: Z) (r1_pre: Z) (l_init: (@list Constraint)) (l2: (@list Constraint)) (l1: (@list Constraint)) (n: Z) (p1: Z) (l3_2: (@list Constraint)) (l4_2: (@list Constraint)) (l11_2: (@list Constraint)) (l12_2: (@list Constraint)) (p1_coef_2: Z) (x: Constraint) (l13: (@list Constraint)) (p2: Z) (p1_next_2: Z) (p1_coef_3: Z) (l3_3: (@list Constraint)) (l4_3: (@list Constraint)) (p1_2: Z) (l21_2: (@list Constraint)) (l22_2: (@list Constraint)) (l11_3: (@list Constraint)) (x1_2: Constraint) (l12_3: (@list Constraint)) (p2_next: Z) (p2_coef: Z) (x_2: Constraint) (l23: (@list Constraint)) (c3: Constraint) (retval_2: Z) (retval: Z) ,
   [| (retval_2 <> 0) |] 
   &&  [| (retval_2 <> 0) |] 
   &&  [| (generate_new_constraint (Zto_nat ((cur_num_pre - 1 ))) x1_2 x_2 c3 ) |] 
   &&  [| (abs_in_int_range (num_pre + 1 ) c3 ) |] 
   &&  [| (l22_2 = (cons (x_2) (l23))) |] 
+  &&  [| (p2_coef <> 0) |] 
   &&  [| (p2 <> 0) |] 
   &&  [| (n = (num_pre + 1 )) |] 
   &&  [| (0 <= cur_num_pre) |] 
@@ -4300,7 +4407,9 @@ forall (cur_num_pre: Z) (num_pre: Z) (r2_pre: Z) (r1_pre: Z) (l_init: (@list Con
   &&  [| (generate_new_constraints_partial (Zto_nat ((cur_num_pre - 1 ))) l11_3 x1_2 l21_2 l22_2 l4_3 ) |] 
   &&  [| (l3_3 = (app (l4_3) (l_init))) |] 
   &&  [| (LP_abs_in_int_range n l3_3 ) |] 
+  &&  [| (p1_coef_3 <> 0) |] 
   &&  [| (l12_2 = (cons (x) (l13))) |] 
+  &&  [| (p1_coef_2 <> 0) |] 
   &&  [| (p1 <> 0) |] 
   &&  [| (n = (num_pre + 1 )) |] 
   &&  [| (0 <= cur_num_pre) |] 
@@ -4321,14 +4430,14 @@ forall (cur_num_pre: Z) (num_pre: Z) (r2_pre: Z) (r1_pre: Z) (l_init: (@list Con
   &&  [| (LP_abs_in_int_range n l2 ) |] 
   &&  [| (LP_abs_in_int_range n l_init ) |]
   &&  (InequList retval n (cons (c3) (l3_3)) )
-  **  (coef_array p1_coef_2 (num_pre + 1 ) x1_2 )
+  **  (coef_array p1_coef_3 (num_pre + 1 ) x1_2 )
   **  (coef_array p2_coef (num_pre + 1 ) x_2 )
-  **  (InequList_seg r2_pre p2 n l21_2 )
   **  ((&((p2)  # "InequList" ->ₛ "coef")) # Ptr  |-> p2_coef)
+  **  (InequList_seg r2_pre p2 n l21_2 )
   **  ((&((p2)  # "InequList" ->ₛ "next")) # Ptr  |-> p2_next)
   **  (InequList p2_next n l23 )
+  **  ((&((p1_2)  # "InequList" ->ₛ "coef")) # Ptr  |-> p1_coef_3)
   **  (InequList_seg r1_pre p1_2 n l11_3 )
-  **  ((&((p1_2)  # "InequList" ->ₛ "coef")) # Ptr  |-> p1_coef_2)
   **  ((&((p1_2)  # "InequList" ->ₛ "next")) # Ptr  |-> p1_next_2)
   **  (InequList p1_next_2 n l12_3 )
 |--
@@ -4344,7 +4453,9 @@ forall (cur_num_pre: Z) (num_pre: Z) (r2_pre: Z) (r1_pre: Z) (l_init: (@list Con
   &&  [| (generate_new_constraints_partial (Zto_nat ((cur_num_pre - 1 ))) l11 x1 l21 l22 l4 ) |] 
   &&  [| (l3 = (app (l4) (l_init))) |] 
   &&  [| (LP_abs_in_int_range n l3 ) |] 
+  &&  [| (p1_coef <> 0) |] 
   &&  [| (l12_2 = (cons (x) (l13))) |] 
+  &&  [| (p1_coef_2 <> 0) |] 
   &&  [| (p1 <> 0) |] 
   &&  [| (n = (num_pre + 1 )) |] 
   &&  [| (0 <= cur_num_pre) |] 
@@ -4364,8 +4475,8 @@ forall (cur_num_pre: Z) (num_pre: Z) (r2_pre: Z) (r1_pre: Z) (l_init: (@list Con
   &&  [| (LP_abs_in_int_range n l1 ) |] 
   &&  [| (LP_abs_in_int_range n l2 ) |] 
   &&  [| (LP_abs_in_int_range n l_init ) |]
-  &&  (InequList_seg r1_pre p1_2 n l11 )
-  **  ((&((p1_2)  # "InequList" ->ₛ "coef")) # Ptr  |-> p1_coef)
+  &&  ((&((p1_2)  # "InequList" ->ₛ "coef")) # Ptr  |-> p1_coef)
+  **  (InequList_seg r1_pre p1_2 n l11 )
   **  (coef_array p1_coef n x1 )
   **  ((&((p1_2)  # "InequList" ->ₛ "next")) # Ptr  |-> p1_next)
   **  (InequList p1_next n l12 )
@@ -4375,7 +4486,7 @@ forall (cur_num_pre: Z) (num_pre: Z) (r2_pre: Z) (r1_pre: Z) (l_init: (@list Con
 .
 
 Definition generate_new_constraint_list_entail_wit_4 := 
-forall (cur_num_pre: Z) (num_pre: Z) (r2_pre: Z) (r1_pre: Z) (l_init: (@list Constraint)) (l2: (@list Constraint)) (l1: (@list Constraint)) (n: Z) (p1_2: Z) (l3_3: (@list Constraint)) (l4_3: (@list Constraint)) (l11_3: (@list Constraint)) (l12_3: (@list Constraint)) (x: Constraint) (l13: (@list Constraint)) (res: Z) (p2: Z) (p1_next: Z) (p1_coef: Z) (l3_2: (@list Constraint)) (l4_2: (@list Constraint)) (p1: Z) (l21: (@list Constraint)) (l22: (@list Constraint)) (l11_2: (@list Constraint)) (x1: Constraint) (l12_2: (@list Constraint)) ,
+forall (cur_num_pre: Z) (num_pre: Z) (r2_pre: Z) (r1_pre: Z) (l_init: (@list Constraint)) (l2: (@list Constraint)) (l1: (@list Constraint)) (n: Z) (p1_2: Z) (l3_3: (@list Constraint)) (l4_3: (@list Constraint)) (l11_3: (@list Constraint)) (l12_3: (@list Constraint)) (p1_coef_2: Z) (x: Constraint) (l13: (@list Constraint)) (res: Z) (p2: Z) (p1_next: Z) (p1_coef: Z) (l3_2: (@list Constraint)) (l4_2: (@list Constraint)) (p1: Z) (l21: (@list Constraint)) (l22: (@list Constraint)) (l11_2: (@list Constraint)) (x1: Constraint) (l12_2: (@list Constraint)) ,
   [| (p2 = 0) |] 
   &&  [| (n = (num_pre + 1 )) |] 
   &&  [| (0 <= cur_num_pre) |] 
@@ -4388,7 +4499,9 @@ forall (cur_num_pre: Z) (num_pre: Z) (r2_pre: Z) (r1_pre: Z) (l_init: (@list Con
   &&  [| (generate_new_constraints_partial (Zto_nat ((cur_num_pre - 1 ))) l11_2 x1 l21 l22 l4_2 ) |] 
   &&  [| (l3_2 = (app (l4_2) (l_init))) |] 
   &&  [| (LP_abs_in_int_range n l3_2 ) |] 
+  &&  [| (p1_coef <> 0) |] 
   &&  [| (l12_3 = (cons (x) (l13))) |] 
+  &&  [| (p1_coef_2 <> 0) |] 
   &&  [| (p1_2 <> 0) |] 
   &&  [| (n = (num_pre + 1 )) |] 
   &&  [| (0 <= cur_num_pre) |] 
@@ -4408,8 +4521,8 @@ forall (cur_num_pre: Z) (num_pre: Z) (r2_pre: Z) (r1_pre: Z) (l_init: (@list Con
   &&  [| (LP_abs_in_int_range n l1 ) |] 
   &&  [| (LP_abs_in_int_range n l2 ) |] 
   &&  [| (LP_abs_in_int_range n l_init ) |]
-  &&  (InequList_seg r1_pre p1 n l11_2 )
-  **  ((&((p1)  # "InequList" ->ₛ "coef")) # Ptr  |-> p1_coef)
+  &&  ((&((p1)  # "InequList" ->ₛ "coef")) # Ptr  |-> p1_coef)
+  **  (InequList_seg r1_pre p1 n l11_2 )
   **  (coef_array p1_coef n x1 )
   **  ((&((p1)  # "InequList" ->ₛ "next")) # Ptr  |-> p1_next)
   **  (InequList p1_next n l12_2 )
@@ -4443,10 +4556,11 @@ forall (cur_num_pre: Z) (num_pre: Z) (r2_pre: Z) (r1_pre: Z) (l_init: (@list Con
 .
 
 Definition generate_new_constraint_list_return_wit_1 := 
-forall (cur_num_pre: Z) (num_pre: Z) (r2_pre: Z) (r1_pre: Z) (l_init: (@list Constraint)) (l2: (@list Constraint)) (l1: (@list Constraint)) (n: Z) (p1: Z) (l3_2: (@list Constraint)) (l4_2: (@list Constraint)) (l11: (@list Constraint)) (l12: (@list Constraint)) (x: Constraint) (l13: (@list Constraint)) (p2: Z) (p1_next: Z) (p1_coef: Z) (l3_3: (@list Constraint)) (l4_3: (@list Constraint)) (p1_2: Z) (l21: (@list Constraint)) (l22: (@list Constraint)) (l11_2: (@list Constraint)) (x1: Constraint) (l12_2: (@list Constraint)) (p2_next: Z) (p2_coef: Z) (x_2: Constraint) (l23: (@list Constraint)) (retval: Z) ,
+forall (cur_num_pre: Z) (num_pre: Z) (r2_pre: Z) (r1_pre: Z) (l_init: (@list Constraint)) (l2: (@list Constraint)) (l1: (@list Constraint)) (n: Z) (p1: Z) (l3_2: (@list Constraint)) (l4_2: (@list Constraint)) (l11: (@list Constraint)) (l12: (@list Constraint)) (p1_coef: Z) (x: Constraint) (l13: (@list Constraint)) (p2: Z) (p1_next: Z) (p1_coef_2: Z) (l3_3: (@list Constraint)) (l4_3: (@list Constraint)) (p1_2: Z) (l21: (@list Constraint)) (l22: (@list Constraint)) (l11_2: (@list Constraint)) (x1: Constraint) (l12_2: (@list Constraint)) (p2_next: Z) (p2_coef: Z) (x_2: Constraint) (l23: (@list Constraint)) (retval: Z) ,
   [| (retval = 0) |] 
   &&  [| (retval = 0) |] 
   &&  [| (l22 = (cons (x_2) (l23))) |] 
+  &&  [| (p2_coef <> 0) |] 
   &&  [| (p2 <> 0) |] 
   &&  [| (n = (num_pre + 1 )) |] 
   &&  [| (0 <= cur_num_pre) |] 
@@ -4459,7 +4573,9 @@ forall (cur_num_pre: Z) (num_pre: Z) (r2_pre: Z) (r1_pre: Z) (l_init: (@list Con
   &&  [| (generate_new_constraints_partial (Zto_nat ((cur_num_pre - 1 ))) l11_2 x1 l21 l22 l4_3 ) |] 
   &&  [| (l3_3 = (app (l4_3) (l_init))) |] 
   &&  [| (LP_abs_in_int_range n l3_3 ) |] 
+  &&  [| (p1_coef_2 <> 0) |] 
   &&  [| (l12 = (cons (x) (l13))) |] 
+  &&  [| (p1_coef <> 0) |] 
   &&  [| (p1 <> 0) |] 
   &&  [| (n = (num_pre + 1 )) |] 
   &&  [| (0 <= cur_num_pre) |] 
@@ -4479,14 +4595,14 @@ forall (cur_num_pre: Z) (num_pre: Z) (r2_pre: Z) (r1_pre: Z) (l_init: (@list Con
   &&  [| (LP_abs_in_int_range n l1 ) |] 
   &&  [| (LP_abs_in_int_range n l2 ) |] 
   &&  [| (LP_abs_in_int_range n l_init ) |]
-  &&  (coef_array p1_coef (num_pre + 1 ) x1 )
+  &&  (coef_array p1_coef_2 (num_pre + 1 ) x1 )
   **  (coef_array p2_coef (num_pre + 1 ) x_2 )
-  **  (InequList_seg r2_pre p2 n l21 )
   **  ((&((p2)  # "InequList" ->ₛ "coef")) # Ptr  |-> p2_coef)
+  **  (InequList_seg r2_pre p2 n l21 )
   **  ((&((p2)  # "InequList" ->ₛ "next")) # Ptr  |-> p2_next)
   **  (InequList p2_next n l23 )
+  **  ((&((p1_2)  # "InequList" ->ₛ "coef")) # Ptr  |-> p1_coef_2)
   **  (InequList_seg r1_pre p1_2 n l11_2 )
-  **  ((&((p1_2)  # "InequList" ->ₛ "coef")) # Ptr  |-> p1_coef)
   **  ((&((p1_2)  # "InequList" ->ₛ "next")) # Ptr  |-> p1_next)
   **  (InequList p1_next n l12_2 )
 |--
@@ -4633,7 +4749,7 @@ forall (cur_num_pre: Z) (num_pre: Z) (r2_pre: Z) (r1_pre: Z) (l_init: (@list Con
 Definition generate_new_constraint_list_partial_solve_wit_1 := generate_new_constraint_list_partial_solve_wit_1_pure -> generate_new_constraint_list_partial_solve_wit_1_aux.
 
 Definition generate_new_constraint_list_partial_solve_wit_2_pure := 
-forall (init_pre: Z) (cur_num_pre: Z) (num_pre: Z) (r2_pre: Z) (r1_pre: Z) (l_init: (@list Constraint)) (l2: (@list Constraint)) (l1: (@list Constraint)) (n: Z) (p1_2: Z) (l3_2: (@list Constraint)) (l4_2: (@list Constraint)) (l11_2: (@list Constraint)) (l12_2: (@list Constraint)) (x: Constraint) (l13: (@list Constraint)) (res: Z) (p2: Z) (p1_next: Z) (p1_coef: Z) (l3: (@list Constraint)) (l4: (@list Constraint)) (p1: Z) (l21: (@list Constraint)) (l22: (@list Constraint)) (l11: (@list Constraint)) (x1: Constraint) (l12: (@list Constraint)) ,
+forall (init_pre: Z) (cur_num_pre: Z) (num_pre: Z) (r2_pre: Z) (r1_pre: Z) (l_init: (@list Constraint)) (l2: (@list Constraint)) (l1: (@list Constraint)) (n: Z) (p1_2: Z) (l3_2: (@list Constraint)) (l4_2: (@list Constraint)) (l11_2: (@list Constraint)) (l12_2: (@list Constraint)) (p1_coef_2: Z) (x: Constraint) (l13: (@list Constraint)) (res: Z) (p2: Z) (p1_next: Z) (p1_coef: Z) (l3: (@list Constraint)) (l4: (@list Constraint)) (p1: Z) (l21: (@list Constraint)) (l22: (@list Constraint)) (l11: (@list Constraint)) (x1: Constraint) (l12: (@list Constraint)) ,
   [| (p2 <> 0) |] 
   &&  [| (n = (num_pre + 1 )) |] 
   &&  [| (0 <= cur_num_pre) |] 
@@ -4646,7 +4762,9 @@ forall (init_pre: Z) (cur_num_pre: Z) (num_pre: Z) (r2_pre: Z) (r1_pre: Z) (l_in
   &&  [| (generate_new_constraints_partial (Zto_nat ((cur_num_pre - 1 ))) l11 x1 l21 l22 l4 ) |] 
   &&  [| (l3 = (app (l4) (l_init))) |] 
   &&  [| (LP_abs_in_int_range n l3 ) |] 
+  &&  [| (p1_coef <> 0) |] 
   &&  [| (l12_2 = (cons (x) (l13))) |] 
+  &&  [| (p1_coef_2 <> 0) |] 
   &&  [| (p1_2 <> 0) |] 
   &&  [| (n = (num_pre + 1 )) |] 
   &&  [| (0 <= cur_num_pre) |] 
@@ -4672,8 +4790,8 @@ forall (init_pre: Z) (cur_num_pre: Z) (num_pre: Z) (r2_pre: Z) (r1_pre: Z) (l_in
   **  ((( &( "r1" ) )) # Ptr  |-> r1_pre)
   **  ((( &( "r2" ) )) # Ptr  |-> r2_pre)
   **  ((( &( "init" ) )) # Ptr  |-> init_pre)
-  **  (InequList_seg r1_pre p1 n l11 )
   **  ((&((p1)  # "InequList" ->ₛ "coef")) # Ptr  |-> p1_coef)
+  **  (InequList_seg r1_pre p1 n l11 )
   **  (coef_array p1_coef n x1 )
   **  ((&((p1)  # "InequList" ->ₛ "next")) # Ptr  |-> p1_next)
   **  (InequList p1_next n l12 )
@@ -4687,7 +4805,7 @@ forall (init_pre: Z) (cur_num_pre: Z) (num_pre: Z) (r2_pre: Z) (r1_pre: Z) (l_in
 .
 
 Definition generate_new_constraint_list_partial_solve_wit_2_aux := 
-forall (cur_num_pre: Z) (num_pre: Z) (r2_pre: Z) (r1_pre: Z) (l_init: (@list Constraint)) (l2: (@list Constraint)) (l1: (@list Constraint)) (n: Z) (p1: Z) (l3: (@list Constraint)) (l4: (@list Constraint)) (l11: (@list Constraint)) (l12: (@list Constraint)) (x: Constraint) (l13: (@list Constraint)) (res: Z) (p2: Z) (p1_next: Z) (p1_coef: Z) (l3_2: (@list Constraint)) (l4_2: (@list Constraint)) (p1_2: Z) (l21: (@list Constraint)) (l22: (@list Constraint)) (l11_2: (@list Constraint)) (x1: Constraint) (l12_2: (@list Constraint)) ,
+forall (cur_num_pre: Z) (num_pre: Z) (r2_pre: Z) (r1_pre: Z) (l_init: (@list Constraint)) (l2: (@list Constraint)) (l1: (@list Constraint)) (n: Z) (p1: Z) (l3: (@list Constraint)) (l4: (@list Constraint)) (l11: (@list Constraint)) (l12: (@list Constraint)) (p1_coef: Z) (x: Constraint) (l13: (@list Constraint)) (res: Z) (p2: Z) (p1_next: Z) (p1_coef_2: Z) (l3_2: (@list Constraint)) (l4_2: (@list Constraint)) (p1_2: Z) (l21: (@list Constraint)) (l22: (@list Constraint)) (l11_2: (@list Constraint)) (x1: Constraint) (l12_2: (@list Constraint)) ,
   [| (p2 <> 0) |] 
   &&  [| (n = (num_pre + 1 )) |] 
   &&  [| (0 <= cur_num_pre) |] 
@@ -4700,7 +4818,9 @@ forall (cur_num_pre: Z) (num_pre: Z) (r2_pre: Z) (r1_pre: Z) (l_init: (@list Con
   &&  [| (generate_new_constraints_partial (Zto_nat ((cur_num_pre - 1 ))) l11_2 x1 l21 l22 l4_2 ) |] 
   &&  [| (l3_2 = (app (l4_2) (l_init))) |] 
   &&  [| (LP_abs_in_int_range n l3_2 ) |] 
+  &&  [| (p1_coef_2 <> 0) |] 
   &&  [| (l12 = (cons (x) (l13))) |] 
+  &&  [| (p1_coef <> 0) |] 
   &&  [| (p1 <> 0) |] 
   &&  [| (n = (num_pre + 1 )) |] 
   &&  [| (0 <= cur_num_pre) |] 
@@ -4720,9 +4840,9 @@ forall (cur_num_pre: Z) (num_pre: Z) (r2_pre: Z) (r1_pre: Z) (l_init: (@list Con
   &&  [| (LP_abs_in_int_range n l1 ) |] 
   &&  [| (LP_abs_in_int_range n l2 ) |] 
   &&  [| (LP_abs_in_int_range n l_init ) |]
-  &&  (InequList_seg r1_pre p1_2 n l11_2 )
-  **  ((&((p1_2)  # "InequList" ->ₛ "coef")) # Ptr  |-> p1_coef)
-  **  (coef_array p1_coef n x1 )
+  &&  ((&((p1_2)  # "InequList" ->ₛ "coef")) # Ptr  |-> p1_coef_2)
+  **  (InequList_seg r1_pre p1_2 n l11_2 )
+  **  (coef_array p1_coef_2 n x1 )
   **  ((&((p1_2)  # "InequList" ->ₛ "next")) # Ptr  |-> p1_next)
   **  (InequList p1_next n l12_2 )
   **  (InequList_seg r2_pre p2 n l21 )
@@ -4742,7 +4862,9 @@ forall (cur_num_pre: Z) (num_pre: Z) (r2_pre: Z) (r1_pre: Z) (l_init: (@list Con
   &&  [| (generate_new_constraints_partial (Zto_nat ((cur_num_pre - 1 ))) l11_2 x1 l21 l22 l4_2 ) |] 
   &&  [| (l3_2 = (app (l4_2) (l_init))) |] 
   &&  [| (LP_abs_in_int_range n l3_2 ) |] 
+  &&  [| (p1_coef_2 <> 0) |] 
   &&  [| (l12 = (cons (x) (l13))) |] 
+  &&  [| (p1_coef <> 0) |] 
   &&  [| (p1 <> 0) |] 
   &&  [| (n = (num_pre + 1 )) |] 
   &&  [| (0 <= cur_num_pre) |] 
@@ -4764,9 +4886,9 @@ forall (cur_num_pre: Z) (num_pre: Z) (r2_pre: Z) (r1_pre: Z) (l_init: (@list Con
   &&  [| (LP_abs_in_int_range n l_init ) |]
   &&  (InequList_seg r2_pre p2 n l21 )
   **  (InequList p2 n l22 )
+  **  ((&((p1_2)  # "InequList" ->ₛ "coef")) # Ptr  |-> p1_coef_2)
   **  (InequList_seg r1_pre p1_2 n l11_2 )
-  **  ((&((p1_2)  # "InequList" ->ₛ "coef")) # Ptr  |-> p1_coef)
-  **  (coef_array p1_coef n x1 )
+  **  (coef_array p1_coef_2 n x1 )
   **  ((&((p1_2)  # "InequList" ->ₛ "next")) # Ptr  |-> p1_next)
   **  (InequList p1_next n l12_2 )
   **  (InequList res n l3_2 )
@@ -4775,8 +4897,9 @@ forall (cur_num_pre: Z) (num_pre: Z) (r2_pre: Z) (r1_pre: Z) (l_init: (@list Con
 Definition generate_new_constraint_list_partial_solve_wit_2 := generate_new_constraint_list_partial_solve_wit_2_pure -> generate_new_constraint_list_partial_solve_wit_2_aux.
 
 Definition generate_new_constraint_list_partial_solve_wit_3_pure := 
-forall (init_pre: Z) (cur_num_pre: Z) (num_pre: Z) (r2_pre: Z) (r1_pre: Z) (l_init: (@list Constraint)) (l2: (@list Constraint)) (l1: (@list Constraint)) (n: Z) (p1: Z) (l3: (@list Constraint)) (l4: (@list Constraint)) (l11: (@list Constraint)) (l12: (@list Constraint)) (x_2: Constraint) (l13: (@list Constraint)) (res: Z) (p2: Z) (p1_next: Z) (p1_coef: Z) (l3_2: (@list Constraint)) (l4_2: (@list Constraint)) (p1_2: Z) (l21: (@list Constraint)) (l22: (@list Constraint)) (l11_2: (@list Constraint)) (x1: Constraint) (l12_2: (@list Constraint)) (p2_next: Z) (p2_coef: Z) (x: Constraint) (l23: (@list Constraint)) ,
+forall (init_pre: Z) (cur_num_pre: Z) (num_pre: Z) (r2_pre: Z) (r1_pre: Z) (l_init: (@list Constraint)) (l2: (@list Constraint)) (l1: (@list Constraint)) (n: Z) (p1: Z) (l3: (@list Constraint)) (l4: (@list Constraint)) (l11: (@list Constraint)) (l12: (@list Constraint)) (p1_coef_2: Z) (x_2: Constraint) (l13: (@list Constraint)) (res: Z) (p2: Z) (p1_next: Z) (p1_coef: Z) (l3_2: (@list Constraint)) (l4_2: (@list Constraint)) (p1_2: Z) (l21: (@list Constraint)) (l22: (@list Constraint)) (l11_2: (@list Constraint)) (x1: Constraint) (l12_2: (@list Constraint)) (p2_next: Z) (p2_coef: Z) (x: Constraint) (l23: (@list Constraint)) ,
   [| (l22 = (cons (x) (l23))) |] 
+  &&  [| (p2_coef <> 0) |] 
   &&  [| (p2 <> 0) |] 
   &&  [| (n = (num_pre + 1 )) |] 
   &&  [| (0 <= cur_num_pre) |] 
@@ -4789,7 +4912,9 @@ forall (init_pre: Z) (cur_num_pre: Z) (num_pre: Z) (r2_pre: Z) (r1_pre: Z) (l_in
   &&  [| (generate_new_constraints_partial (Zto_nat ((cur_num_pre - 1 ))) l11_2 x1 l21 l22 l4_2 ) |] 
   &&  [| (l3_2 = (app (l4_2) (l_init))) |] 
   &&  [| (LP_abs_in_int_range n l3_2 ) |] 
+  &&  [| (p1_coef <> 0) |] 
   &&  [| (l12 = (cons (x_2) (l13))) |] 
+  &&  [| (p1_coef_2 <> 0) |] 
   &&  [| (p1 <> 0) |] 
   &&  [| (n = (num_pre + 1 )) |] 
   &&  [| (0 <= cur_num_pre) |] 
@@ -4811,9 +4936,9 @@ forall (init_pre: Z) (cur_num_pre: Z) (num_pre: Z) (r2_pre: Z) (r1_pre: Z) (l_in
   &&  [| (LP_abs_in_int_range n l_init ) |]
   &&  ((( &( "tmp" ) )) # Ptr  |->_)
   **  ((( &( "p2" ) )) # Ptr  |-> p2)
+  **  ((&((p2)  # "InequList" ->ₛ "coef")) # Ptr  |-> p2_coef)
   **  ((( &( "r2" ) )) # Ptr  |-> r2_pre)
   **  (InequList_seg r2_pre p2 n l21 )
-  **  ((&((p2)  # "InequList" ->ₛ "coef")) # Ptr  |-> p2_coef)
   **  (coef_array p2_coef n x )
   **  ((&((p2)  # "InequList" ->ₛ "next")) # Ptr  |-> p2_next)
   **  (InequList p2_next n l23 )
@@ -4822,8 +4947,8 @@ forall (init_pre: Z) (cur_num_pre: Z) (num_pre: Z) (r2_pre: Z) (r1_pre: Z) (l_in
   **  ((( &( "p1" ) )) # Ptr  |-> p1_2)
   **  ((( &( "r1" ) )) # Ptr  |-> r1_pre)
   **  ((( &( "init" ) )) # Ptr  |-> init_pre)
-  **  (InequList_seg r1_pre p1_2 n l11_2 )
   **  ((&((p1_2)  # "InequList" ->ₛ "coef")) # Ptr  |-> p1_coef)
+  **  (InequList_seg r1_pre p1_2 n l11_2 )
   **  (coef_array p1_coef n x1 )
   **  ((&((p1_2)  # "InequList" ->ₛ "next")) # Ptr  |-> p1_next)
   **  (InequList p1_next n l12_2 )
@@ -4833,6 +4958,8 @@ forall (init_pre: Z) (cur_num_pre: Z) (num_pre: Z) (r2_pre: Z) (r1_pre: Z) (l_in
   [| (0 <= cur_num_pre) |] 
   &&  [| (cur_num_pre < (num_pre + 1 )) |] 
   &&  [| ((num_pre + 1 ) <= INT_MAX) |] 
+  &&  [| (p1_coef <> 0) |] 
+  &&  [| (p2_coef <> 0) |] 
   &&  [| ((-(coef_Znth (cur_num_pre) (x) (0))) <= INT_MAX) |] 
   &&  [| ((coef_Znth (cur_num_pre) (x) (0)) < 0) |] 
   &&  [| ((coef_Znth (cur_num_pre) (x1) (0)) <= INT_MAX) |] 
@@ -4840,8 +4967,9 @@ forall (init_pre: Z) (cur_num_pre: Z) (num_pre: Z) (r2_pre: Z) (r1_pre: Z) (l_in
 .
 
 Definition generate_new_constraint_list_partial_solve_wit_3_aux := 
-forall (cur_num_pre: Z) (num_pre: Z) (r2_pre: Z) (r1_pre: Z) (l_init: (@list Constraint)) (l2: (@list Constraint)) (l1: (@list Constraint)) (n: Z) (p1: Z) (l3: (@list Constraint)) (l4: (@list Constraint)) (l11: (@list Constraint)) (l12: (@list Constraint)) (x: Constraint) (l13: (@list Constraint)) (res: Z) (p2: Z) (p1_next: Z) (p1_coef: Z) (l3_2: (@list Constraint)) (l4_2: (@list Constraint)) (p1_2: Z) (l21: (@list Constraint)) (l22: (@list Constraint)) (l11_2: (@list Constraint)) (x1: Constraint) (l12_2: (@list Constraint)) (p2_next: Z) (p2_coef: Z) (x_2: Constraint) (l23: (@list Constraint)) ,
+forall (cur_num_pre: Z) (num_pre: Z) (r2_pre: Z) (r1_pre: Z) (l_init: (@list Constraint)) (l2: (@list Constraint)) (l1: (@list Constraint)) (n: Z) (p1: Z) (l3: (@list Constraint)) (l4: (@list Constraint)) (l11: (@list Constraint)) (l12: (@list Constraint)) (p1_coef: Z) (x: Constraint) (l13: (@list Constraint)) (res: Z) (p2: Z) (p1_next: Z) (p1_coef_2: Z) (l3_2: (@list Constraint)) (l4_2: (@list Constraint)) (p1_2: Z) (l21: (@list Constraint)) (l22: (@list Constraint)) (l11_2: (@list Constraint)) (x1: Constraint) (l12_2: (@list Constraint)) (p2_next: Z) (p2_coef: Z) (x_2: Constraint) (l23: (@list Constraint)) ,
   [| (l22 = (cons (x_2) (l23))) |] 
+  &&  [| (p2_coef <> 0) |] 
   &&  [| (p2 <> 0) |] 
   &&  [| (n = (num_pre + 1 )) |] 
   &&  [| (0 <= cur_num_pre) |] 
@@ -4854,7 +4982,9 @@ forall (cur_num_pre: Z) (num_pre: Z) (r2_pre: Z) (r1_pre: Z) (l_init: (@list Con
   &&  [| (generate_new_constraints_partial (Zto_nat ((cur_num_pre - 1 ))) l11_2 x1 l21 l22 l4_2 ) |] 
   &&  [| (l3_2 = (app (l4_2) (l_init))) |] 
   &&  [| (LP_abs_in_int_range n l3_2 ) |] 
+  &&  [| (p1_coef_2 <> 0) |] 
   &&  [| (l12 = (cons (x) (l13))) |] 
+  &&  [| (p1_coef <> 0) |] 
   &&  [| (p1 <> 0) |] 
   &&  [| (n = (num_pre + 1 )) |] 
   &&  [| (0 <= cur_num_pre) |] 
@@ -4874,14 +5004,14 @@ forall (cur_num_pre: Z) (num_pre: Z) (r2_pre: Z) (r1_pre: Z) (l_init: (@list Con
   &&  [| (LP_abs_in_int_range n l1 ) |] 
   &&  [| (LP_abs_in_int_range n l2 ) |] 
   &&  [| (LP_abs_in_int_range n l_init ) |]
-  &&  (InequList_seg r2_pre p2 n l21 )
-  **  ((&((p2)  # "InequList" ->ₛ "coef")) # Ptr  |-> p2_coef)
+  &&  ((&((p2)  # "InequList" ->ₛ "coef")) # Ptr  |-> p2_coef)
+  **  (InequList_seg r2_pre p2 n l21 )
   **  (coef_array p2_coef n x_2 )
   **  ((&((p2)  # "InequList" ->ₛ "next")) # Ptr  |-> p2_next)
   **  (InequList p2_next n l23 )
+  **  ((&((p1_2)  # "InequList" ->ₛ "coef")) # Ptr  |-> p1_coef_2)
   **  (InequList_seg r1_pre p1_2 n l11_2 )
-  **  ((&((p1_2)  # "InequList" ->ₛ "coef")) # Ptr  |-> p1_coef)
-  **  (coef_array p1_coef n x1 )
+  **  (coef_array p1_coef_2 n x1 )
   **  ((&((p1_2)  # "InequList" ->ₛ "next")) # Ptr  |-> p1_next)
   **  (InequList p1_next n l12_2 )
   **  (InequList res n l3_2 )
@@ -4889,11 +5019,14 @@ forall (cur_num_pre: Z) (num_pre: Z) (r2_pre: Z) (r1_pre: Z) (l_init: (@list Con
   [| (0 <= cur_num_pre) |] 
   &&  [| (cur_num_pre < (num_pre + 1 )) |] 
   &&  [| ((num_pre + 1 ) <= INT_MAX) |] 
+  &&  [| (p1_coef_2 <> 0) |] 
+  &&  [| (p2_coef <> 0) |] 
   &&  [| ((-(coef_Znth (cur_num_pre) (x_2) (0))) <= INT_MAX) |] 
   &&  [| ((coef_Znth (cur_num_pre) (x_2) (0)) < 0) |] 
   &&  [| ((coef_Znth (cur_num_pre) (x1) (0)) <= INT_MAX) |] 
   &&  [| ((coef_Znth (cur_num_pre) (x1) (0)) > 0) |] 
   &&  [| (l22 = (cons (x_2) (l23))) |] 
+  &&  [| (p2_coef <> 0) |] 
   &&  [| (p2 <> 0) |] 
   &&  [| (n = (num_pre + 1 )) |] 
   &&  [| (0 <= cur_num_pre) |] 
@@ -4906,7 +5039,9 @@ forall (cur_num_pre: Z) (num_pre: Z) (r2_pre: Z) (r1_pre: Z) (l_init: (@list Con
   &&  [| (generate_new_constraints_partial (Zto_nat ((cur_num_pre - 1 ))) l11_2 x1 l21 l22 l4_2 ) |] 
   &&  [| (l3_2 = (app (l4_2) (l_init))) |] 
   &&  [| (LP_abs_in_int_range n l3_2 ) |] 
+  &&  [| (p1_coef_2 <> 0) |] 
   &&  [| (l12 = (cons (x) (l13))) |] 
+  &&  [| (p1_coef <> 0) |] 
   &&  [| (p1 <> 0) |] 
   &&  [| (n = (num_pre + 1 )) |] 
   &&  [| (0 <= cur_num_pre) |] 
@@ -4926,14 +5061,14 @@ forall (cur_num_pre: Z) (num_pre: Z) (r2_pre: Z) (r1_pre: Z) (l_init: (@list Con
   &&  [| (LP_abs_in_int_range n l1 ) |] 
   &&  [| (LP_abs_in_int_range n l2 ) |] 
   &&  [| (LP_abs_in_int_range n l_init ) |]
-  &&  (coef_array p1_coef (num_pre + 1 ) x1 )
+  &&  (coef_array p1_coef_2 (num_pre + 1 ) x1 )
   **  (coef_array p2_coef (num_pre + 1 ) x_2 )
-  **  (InequList_seg r2_pre p2 n l21 )
   **  ((&((p2)  # "InequList" ->ₛ "coef")) # Ptr  |-> p2_coef)
+  **  (InequList_seg r2_pre p2 n l21 )
   **  ((&((p2)  # "InequList" ->ₛ "next")) # Ptr  |-> p2_next)
   **  (InequList p2_next n l23 )
+  **  ((&((p1_2)  # "InequList" ->ₛ "coef")) # Ptr  |-> p1_coef_2)
   **  (InequList_seg r1_pre p1_2 n l11_2 )
-  **  ((&((p1_2)  # "InequList" ->ₛ "coef")) # Ptr  |-> p1_coef)
   **  ((&((p1_2)  # "InequList" ->ₛ "next")) # Ptr  |-> p1_next)
   **  (InequList p1_next n l12_2 )
   **  (InequList res n l3_2 )
@@ -4942,10 +5077,11 @@ forall (cur_num_pre: Z) (num_pre: Z) (r2_pre: Z) (r1_pre: Z) (l_init: (@list Con
 Definition generate_new_constraint_list_partial_solve_wit_3 := generate_new_constraint_list_partial_solve_wit_3_pure -> generate_new_constraint_list_partial_solve_wit_3_aux.
 
 Definition generate_new_constraint_list_partial_solve_wit_4 := 
-forall (cur_num_pre: Z) (num_pre: Z) (r2_pre: Z) (r1_pre: Z) (l_init: (@list Constraint)) (l2: (@list Constraint)) (l1: (@list Constraint)) (n: Z) (p1: Z) (l3: (@list Constraint)) (l4: (@list Constraint)) (l11: (@list Constraint)) (l12: (@list Constraint)) (x: Constraint) (l13: (@list Constraint)) (res: Z) (p2: Z) (p1_next: Z) (p1_coef: Z) (l3_2: (@list Constraint)) (l4_2: (@list Constraint)) (p1_2: Z) (l21: (@list Constraint)) (l22: (@list Constraint)) (l11_2: (@list Constraint)) (x1: Constraint) (l12_2: (@list Constraint)) (p2_next: Z) (p2_coef: Z) (x_2: Constraint) (l23: (@list Constraint)) (retval: Z) ,
+forall (cur_num_pre: Z) (num_pre: Z) (r2_pre: Z) (r1_pre: Z) (l_init: (@list Constraint)) (l2: (@list Constraint)) (l1: (@list Constraint)) (n: Z) (p1: Z) (l3: (@list Constraint)) (l4: (@list Constraint)) (l11: (@list Constraint)) (l12: (@list Constraint)) (p1_coef: Z) (x: Constraint) (l13: (@list Constraint)) (res: Z) (p2: Z) (p1_next: Z) (p1_coef_2: Z) (l3_2: (@list Constraint)) (l4_2: (@list Constraint)) (p1_2: Z) (l21: (@list Constraint)) (l22: (@list Constraint)) (l11_2: (@list Constraint)) (x1: Constraint) (l12_2: (@list Constraint)) (p2_next: Z) (p2_coef: Z) (x_2: Constraint) (l23: (@list Constraint)) (retval: Z) ,
   [| (retval = 0) |] 
   &&  [| (retval = 0) |] 
   &&  [| (l22 = (cons (x_2) (l23))) |] 
+  &&  [| (p2_coef <> 0) |] 
   &&  [| (p2 <> 0) |] 
   &&  [| (n = (num_pre + 1 )) |] 
   &&  [| (0 <= cur_num_pre) |] 
@@ -4958,7 +5094,9 @@ forall (cur_num_pre: Z) (num_pre: Z) (r2_pre: Z) (r1_pre: Z) (l_init: (@list Con
   &&  [| (generate_new_constraints_partial (Zto_nat ((cur_num_pre - 1 ))) l11_2 x1 l21 l22 l4_2 ) |] 
   &&  [| (l3_2 = (app (l4_2) (l_init))) |] 
   &&  [| (LP_abs_in_int_range n l3_2 ) |] 
+  &&  [| (p1_coef_2 <> 0) |] 
   &&  [| (l12 = (cons (x) (l13))) |] 
+  &&  [| (p1_coef <> 0) |] 
   &&  [| (p1 <> 0) |] 
   &&  [| (n = (num_pre + 1 )) |] 
   &&  [| (0 <= cur_num_pre) |] 
@@ -4978,14 +5116,14 @@ forall (cur_num_pre: Z) (num_pre: Z) (r2_pre: Z) (r1_pre: Z) (l_init: (@list Con
   &&  [| (LP_abs_in_int_range n l1 ) |] 
   &&  [| (LP_abs_in_int_range n l2 ) |] 
   &&  [| (LP_abs_in_int_range n l_init ) |]
-  &&  (coef_array p1_coef (num_pre + 1 ) x1 )
+  &&  (coef_array p1_coef_2 (num_pre + 1 ) x1 )
   **  (coef_array p2_coef (num_pre + 1 ) x_2 )
-  **  (InequList_seg r2_pre p2 n l21 )
   **  ((&((p2)  # "InequList" ->ₛ "coef")) # Ptr  |-> p2_coef)
+  **  (InequList_seg r2_pre p2 n l21 )
   **  ((&((p2)  # "InequList" ->ₛ "next")) # Ptr  |-> p2_next)
   **  (InequList p2_next n l23 )
+  **  ((&((p1_2)  # "InequList" ->ₛ "coef")) # Ptr  |-> p1_coef_2)
   **  (InequList_seg r1_pre p1_2 n l11_2 )
-  **  ((&((p1_2)  # "InequList" ->ₛ "coef")) # Ptr  |-> p1_coef)
   **  ((&((p1_2)  # "InequList" ->ₛ "next")) # Ptr  |-> p1_next)
   **  (InequList p1_next n l12_2 )
   **  (InequList res n l3_2 )
@@ -4993,6 +5131,7 @@ forall (cur_num_pre: Z) (num_pre: Z) (r2_pre: Z) (r1_pre: Z) (l_init: (@list Con
   [| (retval = 0) |] 
   &&  [| (retval = 0) |] 
   &&  [| (l22 = (cons (x_2) (l23))) |] 
+  &&  [| (p2_coef <> 0) |] 
   &&  [| (p2 <> 0) |] 
   &&  [| (n = (num_pre + 1 )) |] 
   &&  [| (0 <= cur_num_pre) |] 
@@ -5005,7 +5144,9 @@ forall (cur_num_pre: Z) (num_pre: Z) (r2_pre: Z) (r1_pre: Z) (l_init: (@list Con
   &&  [| (generate_new_constraints_partial (Zto_nat ((cur_num_pre - 1 ))) l11_2 x1 l21 l22 l4_2 ) |] 
   &&  [| (l3_2 = (app (l4_2) (l_init))) |] 
   &&  [| (LP_abs_in_int_range n l3_2 ) |] 
+  &&  [| (p1_coef_2 <> 0) |] 
   &&  [| (l12 = (cons (x) (l13))) |] 
+  &&  [| (p1_coef <> 0) |] 
   &&  [| (p1 <> 0) |] 
   &&  [| (n = (num_pre + 1 )) |] 
   &&  [| (0 <= cur_num_pre) |] 
@@ -5026,25 +5167,26 @@ forall (cur_num_pre: Z) (num_pre: Z) (r2_pre: Z) (r1_pre: Z) (l_init: (@list Con
   &&  [| (LP_abs_in_int_range n l2 ) |] 
   &&  [| (LP_abs_in_int_range n l_init ) |]
   &&  (InequList res n l3_2 )
-  **  (coef_array p1_coef (num_pre + 1 ) x1 )
+  **  (coef_array p1_coef_2 (num_pre + 1 ) x1 )
   **  (coef_array p2_coef (num_pre + 1 ) x_2 )
-  **  (InequList_seg r2_pre p2 n l21 )
   **  ((&((p2)  # "InequList" ->ₛ "coef")) # Ptr  |-> p2_coef)
+  **  (InequList_seg r2_pre p2 n l21 )
   **  ((&((p2)  # "InequList" ->ₛ "next")) # Ptr  |-> p2_next)
   **  (InequList p2_next n l23 )
+  **  ((&((p1_2)  # "InequList" ->ₛ "coef")) # Ptr  |-> p1_coef_2)
   **  (InequList_seg r1_pre p1_2 n l11_2 )
-  **  ((&((p1_2)  # "InequList" ->ₛ "coef")) # Ptr  |-> p1_coef)
   **  ((&((p1_2)  # "InequList" ->ₛ "next")) # Ptr  |-> p1_next)
   **  (InequList p1_next n l12_2 )
 .
 
-Definition generate_new_constraint_list_partial_solve_wit_5 := 
-forall (cur_num_pre: Z) (num_pre: Z) (r2_pre: Z) (r1_pre: Z) (l_init: (@list Constraint)) (l2: (@list Constraint)) (l1: (@list Constraint)) (n: Z) (p1: Z) (l3: (@list Constraint)) (l4: (@list Constraint)) (l11: (@list Constraint)) (l12: (@list Constraint)) (x: Constraint) (l13: (@list Constraint)) (res: Z) (p2: Z) (p1_next: Z) (p1_coef: Z) (l3_2: (@list Constraint)) (l4_2: (@list Constraint)) (p1_2: Z) (l21: (@list Constraint)) (l22: (@list Constraint)) (l11_2: (@list Constraint)) (x1: Constraint) (l12_2: (@list Constraint)) (p2_next: Z) (p2_coef: Z) (x_2: Constraint) (l23: (@list Constraint)) (c3: Constraint) (retval: Z) ,
+Definition generate_new_constraint_list_partial_solve_wit_5_pure := 
+forall (init_pre: Z) (cur_num_pre: Z) (num_pre: Z) (r2_pre: Z) (r1_pre: Z) (l_init: (@list Constraint)) (l2: (@list Constraint)) (l1: (@list Constraint)) (n: Z) (p1: Z) (l3: (@list Constraint)) (l4: (@list Constraint)) (l11: (@list Constraint)) (l12: (@list Constraint)) (p1_coef: Z) (x: Constraint) (l13: (@list Constraint)) (res: Z) (p2: Z) (p1_next: Z) (p1_coef_2: Z) (l3_2: (@list Constraint)) (l4_2: (@list Constraint)) (p1_2: Z) (l21: (@list Constraint)) (l22: (@list Constraint)) (l11_2: (@list Constraint)) (x1: Constraint) (l12_2: (@list Constraint)) (p2_next: Z) (p2_coef: Z) (x_2: Constraint) (l23: (@list Constraint)) (c3: Constraint) (retval: Z) ,
   [| (retval <> 0) |] 
   &&  [| (retval <> 0) |] 
   &&  [| (generate_new_constraint (Zto_nat ((cur_num_pre - 1 ))) x1 x_2 c3 ) |] 
   &&  [| (abs_in_int_range (num_pre + 1 ) c3 ) |] 
   &&  [| (l22 = (cons (x_2) (l23))) |] 
+  &&  [| (p2_coef <> 0) |] 
   &&  [| (p2 <> 0) |] 
   &&  [| (n = (num_pre + 1 )) |] 
   &&  [| (0 <= cur_num_pre) |] 
@@ -5057,7 +5199,9 @@ forall (cur_num_pre: Z) (num_pre: Z) (r2_pre: Z) (r1_pre: Z) (l_init: (@list Con
   &&  [| (generate_new_constraints_partial (Zto_nat ((cur_num_pre - 1 ))) l11_2 x1 l21 l22 l4_2 ) |] 
   &&  [| (l3_2 = (app (l4_2) (l_init))) |] 
   &&  [| (LP_abs_in_int_range n l3_2 ) |] 
+  &&  [| (p1_coef_2 <> 0) |] 
   &&  [| (l12 = (cons (x) (l13))) |] 
+  &&  [| (p1_coef <> 0) |] 
   &&  [| (p1 <> 0) |] 
   &&  [| (n = (num_pre + 1 )) |] 
   &&  [| (0 <= cur_num_pre) |] 
@@ -5077,24 +5221,39 @@ forall (cur_num_pre: Z) (num_pre: Z) (r2_pre: Z) (r1_pre: Z) (l_init: (@list Con
   &&  [| (LP_abs_in_int_range n l1 ) |] 
   &&  [| (LP_abs_in_int_range n l2 ) |] 
   &&  [| (LP_abs_in_int_range n l_init ) |]
-  &&  (coef_array p1_coef (num_pre + 1 ) x1 )
+  &&  (coef_array p1_coef_2 (num_pre + 1 ) x1 )
   **  (coef_array p2_coef (num_pre + 1 ) x_2 )
   **  (coef_array retval (num_pre + 1 ) c3 )
-  **  (InequList_seg r2_pre p2 n l21 )
+  **  ((( &( "tmp" ) )) # Ptr  |-> retval)
+  **  ((( &( "p2" ) )) # Ptr  |-> p2)
   **  ((&((p2)  # "InequList" ->ₛ "coef")) # Ptr  |-> p2_coef)
+  **  ((( &( "r2" ) )) # Ptr  |-> r2_pre)
+  **  (InequList_seg r2_pre p2 n l21 )
   **  ((&((p2)  # "InequList" ->ₛ "next")) # Ptr  |-> p2_next)
   **  (InequList p2_next n l23 )
+  **  ((( &( "num" ) )) # Int  |-> num_pre)
+  **  ((( &( "cur_num" ) )) # Int  |-> cur_num_pre)
+  **  ((( &( "p1" ) )) # Ptr  |-> p1_2)
+  **  ((( &( "r1" ) )) # Ptr  |-> r1_pre)
+  **  ((( &( "init" ) )) # Ptr  |-> init_pre)
+  **  ((&((p1_2)  # "InequList" ->ₛ "coef")) # Ptr  |-> p1_coef_2)
   **  (InequList_seg r1_pre p1_2 n l11_2 )
-  **  ((&((p1_2)  # "InequList" ->ₛ "coef")) # Ptr  |-> p1_coef)
   **  ((&((p1_2)  # "InequList" ->ₛ "next")) # Ptr  |-> p1_next)
   **  (InequList p1_next n l12_2 )
+  **  ((( &( "res" ) )) # Ptr  |-> res)
   **  (InequList res n l3_2 )
 |--
+  [| (retval <> 0) |]
+.
+
+Definition generate_new_constraint_list_partial_solve_wit_5_aux := 
+forall (cur_num_pre: Z) (num_pre: Z) (r2_pre: Z) (r1_pre: Z) (l_init: (@list Constraint)) (l2: (@list Constraint)) (l1: (@list Constraint)) (n: Z) (p1: Z) (l3: (@list Constraint)) (l4: (@list Constraint)) (l11: (@list Constraint)) (l12: (@list Constraint)) (p1_coef: Z) (x: Constraint) (l13: (@list Constraint)) (res: Z) (p2: Z) (p1_next: Z) (p1_coef_2: Z) (l3_2: (@list Constraint)) (l4_2: (@list Constraint)) (p1_2: Z) (l21: (@list Constraint)) (l22: (@list Constraint)) (l11_2: (@list Constraint)) (x1: Constraint) (l12_2: (@list Constraint)) (p2_next: Z) (p2_coef: Z) (x_2: Constraint) (l23: (@list Constraint)) (c3: Constraint) (retval: Z) ,
   [| (retval <> 0) |] 
   &&  [| (retval <> 0) |] 
   &&  [| (generate_new_constraint (Zto_nat ((cur_num_pre - 1 ))) x1 x_2 c3 ) |] 
   &&  [| (abs_in_int_range (num_pre + 1 ) c3 ) |] 
   &&  [| (l22 = (cons (x_2) (l23))) |] 
+  &&  [| (p2_coef <> 0) |] 
   &&  [| (p2 <> 0) |] 
   &&  [| (n = (num_pre + 1 )) |] 
   &&  [| (0 <= cur_num_pre) |] 
@@ -5107,7 +5266,63 @@ forall (cur_num_pre: Z) (num_pre: Z) (r2_pre: Z) (r1_pre: Z) (l_init: (@list Con
   &&  [| (generate_new_constraints_partial (Zto_nat ((cur_num_pre - 1 ))) l11_2 x1 l21 l22 l4_2 ) |] 
   &&  [| (l3_2 = (app (l4_2) (l_init))) |] 
   &&  [| (LP_abs_in_int_range n l3_2 ) |] 
+  &&  [| (p1_coef_2 <> 0) |] 
   &&  [| (l12 = (cons (x) (l13))) |] 
+  &&  [| (p1_coef <> 0) |] 
+  &&  [| (p1 <> 0) |] 
+  &&  [| (n = (num_pre + 1 )) |] 
+  &&  [| (0 <= cur_num_pre) |] 
+  &&  [| (cur_num_pre < n) |] 
+  &&  [| (InequList_nth_pos cur_num_pre l1 ) |] 
+  &&  [| (InequList_nth_neg cur_num_pre l2 ) |] 
+  &&  [| (l1 = (app (l11) (l12))) |] 
+  &&  [| (generate_new_constraints (Zto_nat ((cur_num_pre - 1 ))) l11 l2 l4 ) |] 
+  &&  [| (l3 = (app (l4) (l_init))) |] 
+  &&  [| (LP_abs_in_int_range n l3 ) |] 
+  &&  [| (n = (num_pre + 1 )) |] 
+  &&  [| (0 <= cur_num_pre) |] 
+  &&  [| (cur_num_pre < n) |] 
+  &&  [| (n <= INT_MAX) |] 
+  &&  [| (InequList_nth_pos cur_num_pre l1 ) |] 
+  &&  [| (InequList_nth_neg cur_num_pre l2 ) |] 
+  &&  [| (LP_abs_in_int_range n l1 ) |] 
+  &&  [| (LP_abs_in_int_range n l2 ) |] 
+  &&  [| (LP_abs_in_int_range n l_init ) |]
+  &&  (coef_array p1_coef_2 (num_pre + 1 ) x1 )
+  **  (coef_array p2_coef (num_pre + 1 ) x_2 )
+  **  (coef_array retval (num_pre + 1 ) c3 )
+  **  ((&((p2)  # "InequList" ->ₛ "coef")) # Ptr  |-> p2_coef)
+  **  (InequList_seg r2_pre p2 n l21 )
+  **  ((&((p2)  # "InequList" ->ₛ "next")) # Ptr  |-> p2_next)
+  **  (InequList p2_next n l23 )
+  **  ((&((p1_2)  # "InequList" ->ₛ "coef")) # Ptr  |-> p1_coef_2)
+  **  (InequList_seg r1_pre p1_2 n l11_2 )
+  **  ((&((p1_2)  # "InequList" ->ₛ "next")) # Ptr  |-> p1_next)
+  **  (InequList p1_next n l12_2 )
+  **  (InequList res n l3_2 )
+|--
+  [| (retval <> 0) |] 
+  &&  [| (retval <> 0) |] 
+  &&  [| (retval <> 0) |] 
+  &&  [| (generate_new_constraint (Zto_nat ((cur_num_pre - 1 ))) x1 x_2 c3 ) |] 
+  &&  [| (abs_in_int_range (num_pre + 1 ) c3 ) |] 
+  &&  [| (l22 = (cons (x_2) (l23))) |] 
+  &&  [| (p2_coef <> 0) |] 
+  &&  [| (p2 <> 0) |] 
+  &&  [| (n = (num_pre + 1 )) |] 
+  &&  [| (0 <= cur_num_pre) |] 
+  &&  [| (cur_num_pre < n) |] 
+  &&  [| (InequList_nth_pos cur_num_pre l1 ) |] 
+  &&  [| (InequList_nth_neg cur_num_pre l2 ) |] 
+  &&  [| (l1 = (app (l11_2) ((cons (x1) (l12_2))))) |] 
+  &&  [| (l2 = (app (l21) (l22))) |] 
+  &&  [| (p1_2 <> 0) |] 
+  &&  [| (generate_new_constraints_partial (Zto_nat ((cur_num_pre - 1 ))) l11_2 x1 l21 l22 l4_2 ) |] 
+  &&  [| (l3_2 = (app (l4_2) (l_init))) |] 
+  &&  [| (LP_abs_in_int_range n l3_2 ) |] 
+  &&  [| (p1_coef_2 <> 0) |] 
+  &&  [| (l12 = (cons (x) (l13))) |] 
+  &&  [| (p1_coef <> 0) |] 
   &&  [| (p1 <> 0) |] 
   &&  [| (n = (num_pre + 1 )) |] 
   &&  [| (0 <= cur_num_pre) |] 
@@ -5129,17 +5344,19 @@ forall (cur_num_pre: Z) (num_pre: Z) (r2_pre: Z) (r1_pre: Z) (l_init: (@list Con
   &&  [| (LP_abs_in_int_range n l_init ) |]
   &&  (coef_array retval n c3 )
   **  (InequList res n l3_2 )
-  **  (coef_array p1_coef (num_pre + 1 ) x1 )
+  **  (coef_array p1_coef_2 (num_pre + 1 ) x1 )
   **  (coef_array p2_coef (num_pre + 1 ) x_2 )
-  **  (InequList_seg r2_pre p2 n l21 )
   **  ((&((p2)  # "InequList" ->ₛ "coef")) # Ptr  |-> p2_coef)
+  **  (InequList_seg r2_pre p2 n l21 )
   **  ((&((p2)  # "InequList" ->ₛ "next")) # Ptr  |-> p2_next)
   **  (InequList p2_next n l23 )
+  **  ((&((p1_2)  # "InequList" ->ₛ "coef")) # Ptr  |-> p1_coef_2)
   **  (InequList_seg r1_pre p1_2 n l11_2 )
-  **  ((&((p1_2)  # "InequList" ->ₛ "coef")) # Ptr  |-> p1_coef)
   **  ((&((p1_2)  # "InequList" ->ₛ "next")) # Ptr  |-> p1_next)
   **  (InequList p1_next n l12_2 )
 .
+
+Definition generate_new_constraint_list_partial_solve_wit_5 := generate_new_constraint_list_partial_solve_wit_5_pure -> generate_new_constraint_list_partial_solve_wit_5_aux.
 
 Definition generate_new_constraint_list_which_implies_wit_1 := 
 forall (n: Z) (l12: (@list Constraint)) (l11: (@list Constraint)) (p1: Z) (r1: Z) ,
@@ -5148,9 +5365,10 @@ forall (n: Z) (l12: (@list Constraint)) (l11: (@list Constraint)) (p1: Z) (r1: Z
   **  (InequList p1 n l12 )
 |--
   EX (p1_next: Z)  (p1_coef: Z)  (x: Constraint)  (l13: (@list Constraint)) ,
-  [| (l12 = (cons (x) (l13))) |]
-  &&  (InequList_seg r1 p1 n l11 )
-  **  ((&((p1)  # "InequList" ->ₛ "coef")) # Ptr  |-> p1_coef)
+  [| (l12 = (cons (x) (l13))) |] 
+  &&  [| (p1_coef <> 0) |]
+  &&  ((&((p1)  # "InequList" ->ₛ "coef")) # Ptr  |-> p1_coef)
+  **  (InequList_seg r1 p1 n l11 )
   **  (coef_array p1_coef n x )
   **  ((&((p1)  # "InequList" ->ₛ "next")) # Ptr  |-> p1_next)
   **  (InequList p1_next n l13 )
@@ -5163,9 +5381,10 @@ forall (n: Z) (l22: (@list Constraint)) (l21: (@list Constraint)) (p2: Z) (r2: Z
   **  (InequList p2 n l22 )
 |--
   EX (p2_next: Z)  (p2_coef: Z)  (x: Constraint)  (l23: (@list Constraint)) ,
-  [| (l22 = (cons (x) (l23))) |]
-  &&  (InequList_seg r2 p2 n l21 )
-  **  ((&((p2)  # "InequList" ->ₛ "coef")) # Ptr  |-> p2_coef)
+  [| (l22 = (cons (x) (l23))) |] 
+  &&  [| (p2_coef <> 0) |]
+  &&  ((&((p2)  # "InequList" ->ₛ "coef")) # Ptr  |-> p2_coef)
+  **  (InequList_seg r2 p2 n l21 )
   **  (coef_array p2_coef n x )
   **  ((&((p2)  # "InequList" ->ₛ "next")) # Ptr  |-> p2_next)
   **  (InequList p2_next n l23 )
@@ -7939,16 +8158,11 @@ Axiom proof_of_free_InequList_safety_wit_4 : free_InequList_safety_wit_4.
 Axiom proof_of_free_InequList_return_wit_1 : free_InequList_return_wit_1.
 Axiom proof_of_free_InequList_return_wit_2_1 : free_InequList_return_wit_2_1.
 Axiom proof_of_free_InequList_return_wit_2_2 : free_InequList_return_wit_2_2.
-Axiom proof_of_free_InequList_return_wit_2_3 : free_InequList_return_wit_2_3.
-Axiom proof_of_free_InequList_return_wit_2_4 : free_InequList_return_wit_2_4.
 Axiom proof_of_free_InequList_partial_solve_wit_1 : free_InequList_partial_solve_wit_1.
 Axiom proof_of_free_InequList_partial_solve_wit_2 : free_InequList_partial_solve_wit_2.
 Axiom proof_of_free_InequList_partial_solve_wit_3 : free_InequList_partial_solve_wit_3.
 Axiom proof_of_free_InequList_partial_solve_wit_4 : free_InequList_partial_solve_wit_4.
 Axiom proof_of_free_InequList_partial_solve_wit_5 : free_InequList_partial_solve_wit_5.
-Axiom proof_of_free_InequList_partial_solve_wit_6 : free_InequList_partial_solve_wit_6.
-Axiom proof_of_free_InequList_partial_solve_wit_7 : free_InequList_partial_solve_wit_7.
-Axiom proof_of_free_InequList_partial_solve_wit_8 : free_InequList_partial_solve_wit_8.
 Axiom proof_of_eliminate_safety_wit_1 : eliminate_safety_wit_1.
 Axiom proof_of_eliminate_safety_wit_2 : eliminate_safety_wit_2.
 Axiom proof_of_eliminate_safety_wit_3 : eliminate_safety_wit_3.
@@ -8041,6 +8255,7 @@ Axiom proof_of_generate_new_constraint_list_partial_solve_wit_2 : generate_new_c
 Axiom proof_of_generate_new_constraint_list_partial_solve_wit_3_pure : generate_new_constraint_list_partial_solve_wit_3_pure.
 Axiom proof_of_generate_new_constraint_list_partial_solve_wit_3 : generate_new_constraint_list_partial_solve_wit_3.
 Axiom proof_of_generate_new_constraint_list_partial_solve_wit_4 : generate_new_constraint_list_partial_solve_wit_4.
+Axiom proof_of_generate_new_constraint_list_partial_solve_wit_5_pure : generate_new_constraint_list_partial_solve_wit_5_pure.
 Axiom proof_of_generate_new_constraint_list_partial_solve_wit_5 : generate_new_constraint_list_partial_solve_wit_5.
 Axiom proof_of_generate_new_constraint_list_which_implies_wit_1 : generate_new_constraint_list_which_implies_wit_1.
 Axiom proof_of_generate_new_constraint_list_which_implies_wit_2 : generate_new_constraint_list_which_implies_wit_2.
