QCP/SeparationLogic/examples/fme/fme_proof_auto.v
@@ -83,7 +83,7 @@ Proof. Admitted.
 Lemma proof_of_free_InequList_safety_wit_4 : free_InequList_safety_wit_4.
 Proof. Admitted. 
 
-Lemma proof_of_free_InequList_return_wit_2_2 : free_InequList_return_wit_2_2.
+Lemma proof_of_free_InequList_return_wit_2_1 : free_InequList_return_wit_2_1.
 Proof. Admitted. 
 
 Lemma proof_of_free_InequList_partial_solve_wit_1 : free_InequList_partial_solve_wit_1.
@@ -99,15 +99,6 @@ Lemma proof_of_free_InequList_partial_solve_wit_4 : free_InequList_partial_solve
 Proof. Admitted. 
 
 Lemma proof_of_free_InequList_partial_solve_wit_5 : free_InequList_partial_solve_wit_5.
-Proof. Admitted. 
-
-Lemma proof_of_free_InequList_partial_solve_wit_6 : free_InequList_partial_solve_wit_6.
-Proof. Admitted. 
-
-Lemma proof_of_free_InequList_partial_solve_wit_7 : free_InequList_partial_solve_wit_7.
-Proof. Admitted. 
-
-Lemma proof_of_free_InequList_partial_solve_wit_8 : free_InequList_partial_solve_wit_8.
 Proof. Admitted. 
 
 Lemma proof_of_eliminate_safety_wit_1 : eliminate_safety_wit_1.
@@ -306,6 +297,9 @@ Lemma proof_of_generate_new_constraint_list_partial_solve_wit_3 : generate_new_c
 Proof. Admitted. 
 
 Lemma proof_of_generate_new_constraint_list_partial_solve_wit_4 : generate_new_constraint_list_partial_solve_wit_4.
+Proof. Admitted. 
+
+Lemma proof_of_generate_new_constraint_list_partial_solve_wit_5_pure : generate_new_constraint_list_partial_solve_wit_5_pure.
 Proof. Admitted. 
 
 Lemma proof_of_generate_new_constraint_list_partial_solve_wit_5 : generate_new_constraint_list_partial_solve_wit_5.
