QCP/SeparationLogic/examples/fme/fme_strategy_goal.v
@@ -129,10 +129,11 @@ Definition fme_strategy13 :=
       ).
 
 Definition fme_strategy15 :=
-  forall (i : Z) (n : Z) (p : Z) (l : Constraint),
+  forall (p : Z) (n : Z) (i : Z) (l : Constraint),
     TT &&
     ([| (Z.le 0 i) |]) &&
     ([| (Z.lt i n) |]) &&
+    ([| (p <> 0) |]) &&
     emp **
     ((coef_array p n l))
     |--
@@ -151,10 +152,11 @@ Definition fme_strategy15 :=
       ).
 
 Definition fme_strategy16 :=
-  forall (i : Z) (n : Z) (l : Constraint) (p : Z),
+  forall (p : Z) (n : Z) (i : Z) (l : Constraint),
     TT &&
     ([| (Z.le 0 i) |]) &&
     ([| (Z.lt i n) |]) &&
+    ([| (p <> 0) |]) &&
     emp **
     ((coef_array_missing_i_rec p i 0 n l)) **
     ((poly_store FET_int (Z.add p (Z.mul i (@sizeof_front_end_type FET_int))) ( coef_Znth i l 0)))
@@ -221,6 +223,7 @@ Definition fme_strategy11 :=
     EX (y : Z) (h : Z),
       (
       TT &&
+      ([| (h <> 0) |]) &&
       emp **
       ((poly_store FET_ptr &( ((p)) # "InequList" ->ₛ "coef") h)) **
       ((coef_array h n x)) **
@@ -246,6 +249,7 @@ Definition fme_strategy12 :=
     ) ** (
     ALL (h : Z) (x : Constraint) (y : Z) (l : (@list Constraint)) (n : Z),
       TT &&
+      ([| (h <> 0) |]) &&
       emp **
       ((poly_store FET_ptr &( ((p)) # "InequList" ->ₛ "coef") h)) **
       ((coef_array h n x)) **
@@ -257,10 +261,11 @@ Definition fme_strategy12 :=
       ).
 
 Definition fme_strategy17 :=
-  forall (i : Z) (n : Z) (l : Constraint) (v : Z) (p : Z),
+  forall (p : Z) (n : Z) (i : Z) (l : Constraint) (v : Z),
     TT &&
     ([| (Z.le 1 i) |]) &&
     ([| (Z.lt i n) |]) &&
+    ([| (p <> 0) |]) &&
     emp **
     ((coef_array_missing_i_rec p i 0 n l)) **
     ((poly_store FET_int (Z.add p (Z.mul i (@sizeof_front_end_type FET_int))) v))
