QCP/SeparationLogic/examples/simple_arith/Always_pos_goal.v
@@ -17,8 +17,8 @@ Local Open Scope list.
 Import naive_C_Rules.
 Require Import Apos_lib.
 Local Open Scope sac.
-From SimpleC.EE Require Import common_strategy_goal.
-From SimpleC.EE Require Import common_strategy_proof.
+Require Import common_strategy_goal.
+Require Import common_strategy_proof.
 
 (*----- Function Always_positive_simple -----*)
 
